WIP2

coq/UntypedSemantics.v
@@ -1,6 +1,6 @@
 (*! Language | Semantics of typed Kôika programs !*)
 Require Export Koika.Common Koika.Environments Koika.ULogs Koika.Syntax
-  Koika.Syntax.
+        Koika.Syntax.
 
 
 Ltac destr_in H :=
@@ -43,41 +43,14 @@ Section Interp.
     context (fun k_tau => uaction) argspec.
 
   Section Action.
-    Context (r: REnv.(env_t) (fun _ => val)).
-    Context (sigma: forall f, Sig_denote (Sigma f)).
-
-    (* Section Args. *)
-    (*   Context (interp_action: *)
-    (*              forall {sig: tsig var_t} {tau} *)
-    (*                (Gamma: tcontext sig) *)
-    (*                (sched_log: Log) (action_log: Log) *)
-    (*                (a: action sig tau), *)
-    (*                option (Log * type_denote tau * (tcontext sig))). *)
-
-    (*   Fixpoint interp_args' *)
-    (*            {sig: tsig var_t} *)
-    (*            (Gamma: tcontext sig) *)
-    (*            (sched_log: Log) *)
-    (*            (action_log: Log) *)
-    (*            {argspec: tsig var_t} *)
-    (*            (args: acontext sig argspec) *)
-    (*     : option (Log * tcontext argspec * (tcontext sig)) := *)
-    (*     match args with *)
-    (*     | CtxEmpty => Some (action_log, CtxEmpty, Gamma) *)
-    (*     | @CtxCons _ _ argspec k_tau arg args => *)
-    (*       let/opt3 action_log, ctx, Gamma := interp_args' Gamma sched_log action_log args in *)
-    (*       let/opt3 action_log, v, Gamma := interp_action _ _ Gamma sched_log action_log arg in *)
-    (*       Some (action_log, CtxCons k_tau v ctx, Gamma) *)
-    (*     end. *)
-    (* End Args. *)
 
     Fixpoint ucassoc {sig: tsig var_t} (Gamma: tcontext sig) (k: var_t)
       : option val
-    :=
-      match Gamma with
-      | CtxEmpty => None
-      | CtxCons k' v Gamma => if eq_dec k (fst k') then Some v else ucassoc Gamma k
-      end.
+      :=
+        match Gamma with
+        | CtxEmpty => None
+        | CtxCons k' v Gamma => if eq_dec k (fst k') then Some v else ucassoc Gamma k
+        end.
 
     Lemma cassoc_ucassoc:
       forall (sig: tsig var_t) (ND: NoDup (map fst sig)) (Gamma: tcontext sig) k,
@@ -89,8 +62,8 @@ Section Interp.
       destruct k, k0; simpl in *. subst.
       inversion m; subst.
       generalize (
-        fun nd => member_NoDup (v0, t) (EqDec_pair _ _) nd m (MemberHd _ _)
-      ).
+          fun nd => member_NoDup (v0, t) (EqDec_pair _ _) nd m (MemberHd _ _)
+        ).
       intros. rewrite H. simpl. auto. apply NoDup_map_inv with (f:= fst).
       simpl; auto.
       apply member_In in X. inversion ND. subst. exfalso; apply H1.
@@ -181,14 +154,14 @@ Section Interp.
 
     Fixpoint replace {sig: tsig var_t} k (v: val) (Gamma: tcontext sig)
       : tcontext sig
-    :=
-      match Gamma with
-      | CtxEmpty => CtxEmpty
-      | CtxCons k0 v0 Gamma =>
-        if eq_dec k (fst k0)
-        then CtxCons k0 v Gamma
-        else CtxCons k0 v0 (replace k v Gamma)
-      end.
+      :=
+        match Gamma with
+        | CtxEmpty => CtxEmpty
+        | CtxCons k0 v0 Gamma =>
+          if eq_dec k (fst k0)
+          then CtxCons k0 v Gamma
+          else CtxCons k0 v0 (replace k v Gamma)
+        end.
 
     Definition bits_split (n: nat) {sz} (v: bits sz)
       : option (bits n * bits (sz - n)).
@@ -219,14 +192,14 @@ Section Interp.
 
     Fixpoint bits_splitn (nb sz_elt: nat) (bs: list bool)
       : option (list (list bool))
-    :=
-      match nb with
-        O => Some []
-      | S nb =>
-        let/opt2 hd, rest := take_drop sz_elt bs in
-        let/opt tl := bits_splitn nb sz_elt rest in
-        Some (hd :: tl)
-      end.
+      :=
+        match nb with
+          O => Some []
+        | S nb =>
+          let/opt2 hd, rest := take_drop sz_elt bs in
+          let/opt tl := bits_splitn nb sz_elt rest in
+          Some (hd :: tl)
+        end.
 
     Lemma take_drop_succeeds:
       forall {A:Type} (n: nat) (l: list A) (LT: n <= Datatypes.length l),
@@ -256,8 +229,8 @@ Section Interp.
 
     Lemma take_drop'_cons:
       forall {A} (l l1 l2: list A) a n,
-      take_drop' n l = (l1, l2) ->
-      take_drop' (S n) (a::l) = (a::l1, l2).
+        take_drop' n l = (l1, l2) ->
+        take_drop' (S n) (a::l) = (a::l1, l2).
     Proof.
       unfold take_drop'. simpl. intros. destruct (take_drop n l) eqn:?.
       - destruct p. inversion H; subst. simpl. auto.
@@ -321,17 +294,17 @@ Section Interp.
 
     Lemma wt_val_ind':
       forall (P : type -> val -> Prop)
-       (Hbits: forall (n : nat) (bs : list bool), Datatypes.length bs = n -> P (bits_t n) (Bits n bs))
-       (Henum: forall (sig : enum_sig) (bs : list bool),
-        Datatypes.length bs = enum_bitsize sig -> P (enum_t sig) (Enum sig bs))
-       (Hstruct: forall (sig : struct_sig) (lv : list val),
-        Forall2 (fun (nt : type) (v : val) => wt_val nt v) (map snd (struct_fields sig)) lv ->
-        Forall2 (fun (nt : type) (v : val) => wt_val nt v -> P nt v) (map snd (struct_fields sig)) lv ->
-        P (struct_t sig) (Struct sig lv))
-       (Harray: forall (sig : array_sig) (lv : list val),
-        Forall (fun v : val => wt_val (array_type sig) v) lv ->
-        Forall (fun v : val => wt_val (array_type sig) v -> P (array_type sig) v) lv ->
-        Datatypes.length lv = array_len sig -> P (array_t sig) (Array sig lv)),
+             (Hbits: forall (n : nat) (bs : list bool), Datatypes.length bs = n -> P (bits_t n) (Bits n bs))
+             (Henum: forall (sig : enum_sig) (bs : list bool),
+                 Datatypes.length bs = enum_bitsize sig -> P (enum_t sig) (Enum sig bs))
+             (Hstruct: forall (sig : struct_sig) (lv : list val),
+                 Forall2 (fun (nt : type) (v : val) => wt_val nt v) (map snd (struct_fields sig)) lv ->
+                 Forall2 (fun (nt : type) (v : val) => wt_val nt v -> P nt v) (map snd (struct_fields sig)) lv ->
+                 P (struct_t sig) (Struct sig lv))
+             (Harray: forall (sig : array_sig) (lv : list val),
+                 Forall (fun v : val => wt_val (array_type sig) v) lv ->
+                 Forall (fun v : val => wt_val (array_type sig) v -> P (array_type sig) v) lv ->
+                 Datatypes.length lv = array_len sig -> P (array_t sig) (Array sig lv)),
       forall (t : type) (v : val), wt_val t v -> P t v.
     Proof.
       intros P Hbits Henum Hstruct Harray t v.
@@ -454,29 +427,29 @@ Section Interp.
 
     Fixpoint uvalue_of_bits {tau: type} (bs: list bool) {struct tau}: option val :=
       let uvalue_of_struct_bits :=
-        (fix uvalue_of_struct_bits
-             {fields: list (string * type)}
-             (bs: list bool)
-         : option (list val) :=
-           match fields with
-           | [] => Some []
-           | (nm, tau) :: fields =>
-             let/opt2 b0, b1 := take_drop (List.length bs - type_sz tau) bs in
-             let/opt tl := uvalue_of_struct_bits (fields:=fields) b0 in
-             let/opt hd := uvalue_of_bits (tau:=tau) b1 in
-             Some ( hd :: tl)
-           end) in
+          (fix uvalue_of_struct_bits
+               {fields: list (string * type)}
+               (bs: list bool)
+           : option (list val) :=
+             match fields with
+             | [] => Some []
+             | (nm, tau) :: fields =>
+               let/opt2 b0, b1 := take_drop (List.length bs - type_sz tau) bs in
+               let/opt tl := uvalue_of_struct_bits (fields:=fields) b0 in
+               let/opt hd := uvalue_of_bits (tau:=tau) b1 in
+               Some ( hd :: tl)
+             end) in
       let uvalue_of_list_bits tau :=
-        fix uvalue_of_list_bits (l : list (list bool))
+          fix uvalue_of_list_bits (l : list (list bool))
           : option (list val)
-        :=
-          match l with
-          | [] => Some []
-          | hd::tl =>
-            let/opt hd := uvalue_of_bits (tau:=tau) hd in
-            let/opt tl := uvalue_of_list_bits tl in
-            Some (hd::tl)
-          end in
+            :=
+              match l with
+              | [] => Some []
+              | hd::tl =>
+                let/opt hd := uvalue_of_bits (tau:=tau) hd in
+                let/opt tl := uvalue_of_list_bits tl in
+                Some (hd::tl)
+              end in
       match tau with
       | bits_t _ => Some (Bits (Datatypes.length bs) bs)
       | enum_t sig =>
@@ -531,12 +504,12 @@ Section Interp.
         simpl.
         rewrite rev_involutive.
         cut ((fix uvalue_of_list_bits (l : list (list bool)) : option (list val) :=
-         match l with
-         | [] => Some []
-         | hd :: tl =>
-             let/opt hd0 := uvalue_of_bits (tau:=array_type sig) hd
-             in (let/opt tl0 := uvalue_of_list_bits tl in Some (hd0 :: tl0))
-         end) ((map ubits_of_value lv)) = Some lv).
+                match l with
+                | [] => Some []
+                | hd :: tl =>
+                  let/opt hd0 := uvalue_of_bits (tau:=array_type sig) hd
+                  in (let/opt tl0 := uvalue_of_list_bits tl in Some (hd0 :: tl0))
+                end) ((map ubits_of_value lv)) = Some lv).
         intro A; rewrite A. simpl. reflexivity.
         revert H1 H2. generalize lv (array_len sig). clear.
         intros l n EQ. subst. revert l.
@@ -549,32 +522,6 @@ Section Interp.
         erewrite ubits_of_value_len'. eauto.
         apply H2. auto. rewrite rev_length, map_length; auto.
     Qed.
-
-    (* Lemma struct_eq: *)
-    (*   forall fields x, *)
-    (*     rev ((fix *)
-    (*            val_of_struct_value (fields : list (string * type)) (x : struct_denote fields) {struct *)
-    (*                                                                                              fields} : list val := *)
-    (*            match fields as fields0 return (struct_denote fields0 -> list val) with *)
-    (*            | [] => fun _ : unit => [] *)
-    (*            | p :: fields0 => *)
-    (*              let (_, tau) as p0 return (snd p0 * struct_denote fields0 -> list val) := p in *)
-    (*              fun '(x0, xs) => val_of_value x0 :: val_of_struct_value fields0 xs *)
-    (*            end x) fields x) =  *)
-    (*     (fix *)
-    (*        val_of_struct_value (fields : list (string * type)) (x : struct_denote fields) {struct *)
-    (*                                                                                          fields} : list val := *)
-    (*        match fields as fields0 return (struct_denote fields0 -> list val) with *)
-    (*        | [] => fun _ : unit => [] *)
-    (*        | p :: fields0 => *)
-    (*          let (_, tau) as p0 return (snd p0 * struct_denote fields0 -> list val) := p in *)
-    (*          fun '(x0, xs) => [val_of_value x0] ++ val_of_struct_value fields0 xs *)
-    (*        end x) fields x. *)
-    (* Proof. *)
-    (*   induction fields. reflexivity. intros. *)
-    (*   destruct a. destruct x. *)
-    (*   rewrite rev_app_distr. simpl. f_equal. eauto. *)
-    (* Qed. *)
 
     Lemma wt_val_of_value:
       forall (tau: type) (v: tau),
@@ -648,17 +595,6 @@ Section Interp.
       | _, _ => None
       end.
 
-    (* Fixpoint find_field (s: list (string * type)) f : option (nat * nat) := *)
-    (*   match s with *)
-    (*   | (n, t)::s => *)
-    (*     if eq_dec f n *)
-    (*     then Some (0, type_sz t) *)
-    (*     else *)
-    (*       let/opt2 ofs, sz := find_field s f in *)
-    (*       Some (ofs + type_sz t, sz) *)
-    (*   | _ => None *)
-    (*   end. *)
-
 
     Fixpoint find_field_offset_right (s: list (string * type)) f : option (nat * nat) :=
       match s with
@@ -670,8 +606,6 @@ Section Interp.
           find_field_offset_right s f
       | [] => None
       end.
-
-
 
     Definition get_field (s: val) f : option val :=
       match s with
@@ -720,123 +654,157 @@ Section Interp.
       end.
 
 
-Lemma uvalue_of_bits_val_of_value:
-  forall (tau: type) (v: vect bool (type_sz tau)),
-    uvalue_of_bits (tau:=tau) (vect_to_list v) = Some (val_of_value (value_of_bits v)).
-Proof.
-  intros; rewrite <- uvalue_of_bits_val'. f_equal.
-  erewrite <- ubits_of_value_ok. 2: eauto.
-  rewrite bits_of_value_of_bits. auto.
-Qed.
+    Lemma uvalue_of_bits_val_of_value:
+      forall (tau: type) (v: vect bool (type_sz tau)),
+        uvalue_of_bits (tau:=tau) (vect_to_list v) = Some (val_of_value (value_of_bits v)).
+    Proof.
+      intros; rewrite <- uvalue_of_bits_val'. f_equal.
+      erewrite <- ubits_of_value_ok. 2: eauto.
+      rewrite bits_of_value_of_bits. auto.
+    Qed.
 
-Lemma repeat_bits_const:
-  forall x n,
-    repeat x n = vect_to_list (Bits.const n x).
-Proof.
-  induction n; simpl; auto.
-  rewrite IHn. reflexivity.
-Qed.
+    Lemma repeat_bits_const:
+      forall x n,
+        repeat x n = vect_to_list (Bits.const n x).
+    Proof.
+      induction n; simpl; auto.
+      rewrite IHn. reflexivity.
+    Qed.
 
-Lemma last_nth:
-  forall {A} d (l: list A),
-    last l d = nth (List.length l - 1) l d.
-Proof.
-  induction l; simpl; intros; eauto.
-  destr. simpl. auto.
-  rewrite IHl. simpl. rewrite Nat.sub_0_r. reflexivity.
-Qed.
+    Lemma last_nth:
+      forall {A} d (l: list A),
+        last l d = nth (List.length l - 1) l d.
+    Proof.
+      induction l; simpl; intros; eauto.
+      destr. simpl. auto.
+      rewrite IHl. simpl. rewrite Nat.sub_0_r. reflexivity.
+    Qed.
 
-Lemma bits_nth_list:
-  forall s (v: vect bool s) idx,
-    Bits.nth v idx = nth (index_to_nat idx) (vect_to_list v) false.
-Proof.
-  induction s; intros. simpl in idx; easy.
-  unfold Bits.nth. destr. simpl. auto. fold @vect_nth.
-  rewrite IHs. destruct v.  simpl. reflexivity.
-Qed.
+    Lemma bits_nth_list:
+      forall s (v: vect bool s) idx,
+        Bits.nth v idx = nth (index_to_nat idx) (vect_to_list v) false.
+    Proof.
+      induction s; intros. simpl in idx; easy.
+      unfold Bits.nth. destr. simpl. auto. fold @vect_nth.
+      rewrite IHs. destruct v.  simpl. reflexivity.
+    Qed.
 
-Lemma msb_spec:
-  forall s (v: bits s),
-    Bits.msb v = last (vect_to_list v) false.
-Proof.
-  unfold Bits.msb. intros.
-  destr. destruct v. reflexivity.
-  rewrite vect_last_nth.
-  rewrite last_nth. rewrite vect_to_list_length.
-  simpl Nat.sub.
-  rewrite Nat.sub_0_r.
-  rewrite bits_nth_list. f_equal.
-  apply index_to_nat_of_nat.
-  apply index_of_nat_largest.
-Qed.
-
-
-          Lemma vect_extend_end_firstn:
-            forall x s' (v: bits (Nat.min x s')) d,
-              vect_to_list (vect_extend_end_firstn v d) =
-              vect_to_list (vect_extend_end v x d).
-          Proof.
-            unfold vect_extend_end_firstn.
-            intros. rewrite vect_to_list_eq_rect. auto.
-          Qed.
-
-          Lemma vect_to_list_cons:
-            forall e s (v: bits s),
-              vect_to_list (v~e) = e:: vect_to_list v.
-          Proof.
-            reflexivity.
-          Qed.
-
-          Lemma vect_firstn_to_list:
-            forall s (v: bits s) n,
-              vect_to_list (vect_firstn n v) = fst (take_drop' n (vect_to_list v)).
-          Proof.
-            induction s; simpl; intros. simpl in *. destruct v. destr; reflexivity.
-            destr. reflexivity.
-            erewrite <- vect_to_list_eq_rect.
-            Unshelve.
-            3: replace (Nat.min (S n0) (S s)) with (S (Nat.min n0 s)); reflexivity.
-            simpl.
-            rewrite vect_to_list_cons.
-            rewrite IHs.
-            destruct v. simpl.
-            cbn. unfold take_drop'. simpl. unfold vect_to_list.
-            destr. destruct p. simpl. reflexivity.
-            simpl. reflexivity.
-          Qed.
-
-          Lemma vect_skipn_to_list:
-            forall s (v: bits s) n,
-              vect_to_list (vect_skipn n v) = snd (take_drop' n (vect_to_list v)).
-          Proof.
-            induction s; simpl; intros. simpl in *. destruct v. destr; reflexivity.
-            destr. reflexivity.
-            rewrite IHs.
-            unfold take_drop'.
-            destruct v. simpl.
-            cbn. unfold vect_to_list.
-            destr. destruct p. simpl. reflexivity.
-            simpl. reflexivity.
-          Qed.
-
-          Lemma take_drop'_spec2:
-            forall {A:Type} (n: nat) (l la lb: list A),
-              take_drop' n l = (la, lb) ->
-              l = la ++ lb /\
-              List.length la = Nat.min n (List.length l).
-          Proof.
-            induction n; simpl; intros; eauto.
-            inversion H; clear H; subst. repeat split; try reflexivity.
-            destruct l; simpl in *. unfold take_drop' in H. simpl in *. inversion H; clear H.
-            simpl. repeat split; lia.
-            destruct (take_drop' n l) as (l1 & l2) eqn:?.
-            erewrite take_drop'_cons in H; eauto. inv H. simpl.
-            apply IHn in Heqp. destruct Heqp as (EQ1 & EQ2). subst.
-            repeat split; auto.
-          Qed.
+    Lemma msb_spec:
+      forall s (v: bits s),
+        Bits.msb v = last (vect_to_list v) false.
+    Proof.
+      unfold Bits.msb. intros.
+      destr. destruct v. reflexivity.
+      rewrite vect_last_nth.
+      rewrite last_nth. rewrite vect_to_list_length.
+      simpl Nat.sub.
+      rewrite Nat.sub_0_r.
+      rewrite bits_nth_list. f_equal.
+      apply index_to_nat_of_nat.
+      apply index_of_nat_largest.
+    Qed.
 
 
-Lemma usigma1_correct:
+    Lemma vect_extend_end_firstn:
+      forall x s' (v: bits (Nat.min x s')) d,
+        vect_to_list (vect_extend_end_firstn v d) =
+        vect_to_list (vect_extend_end v x d).
+    Proof.
+      unfold vect_extend_end_firstn.
+      intros. rewrite vect_to_list_eq_rect. auto.
+    Qed.
+
+    Lemma vect_to_list_cons:
+      forall {A: Type} e s (v: vect A s),
+        vect_to_list (e::v)%vect = e:: vect_to_list v.
+    Proof.
+      reflexivity.
+    Qed.
+
+    Lemma vect_firstn_to_list:
+      forall s (v: bits s) n,
+        vect_to_list (vect_firstn n v) = fst (take_drop' n (vect_to_list v)).
+    Proof.
+      induction s; simpl; intros. simpl in *. destruct v. destr; reflexivity.
+      destr. reflexivity.
+      erewrite <- vect_to_list_eq_rect.
+      Unshelve.
+      3: replace (Nat.min (S n0) (S s)) with (S (Nat.min n0 s)); reflexivity.
+      simpl.
+      rewrite vect_to_list_cons.
+      rewrite IHs.
+      destruct v. simpl.
+      cbn. unfold take_drop'. simpl. unfold vect_to_list.
+      destr. destruct p. simpl. reflexivity.
+      simpl. reflexivity.
+    Qed.
+
+    Lemma vect_skipn_to_list:
+      forall s (v: bits s) n,
+        vect_to_list (vect_skipn n v) = snd (take_drop' n (vect_to_list v)).
+    Proof.
+      induction s; simpl; intros. simpl in *. destruct v. destr; reflexivity.
+      destr. reflexivity.
+      rewrite IHs.
+      unfold take_drop'.
+      destruct v. simpl.
+      cbn. unfold vect_to_list.
+      destr. destruct p. simpl. reflexivity.
+      simpl. reflexivity.
+    Qed.
+
+    Lemma take_drop'_spec2:
+      forall {A:Type} (n: nat) (l la lb: list A),
+        take_drop' n l = (la, lb) ->
+        l = la ++ lb /\
+        List.length la = Nat.min n (List.length l).
+    Proof.
+      induction n; simpl; intros; eauto.
+      inversion H; clear H; subst. repeat split; try reflexivity.
+      destruct l; simpl in *. unfold take_drop' in H. simpl in *. inversion H; clear H.
+      simpl. repeat split; lia.
+      destruct (take_drop' n l) as (l1 & l2) eqn:?.
+      erewrite take_drop'_cons in H; eauto. inv H. simpl.
+      apply IHn in Heqp. destruct Heqp as (EQ1 & EQ2). subst.
+      repeat split; auto.
+    Qed.
+
+    Lemma struct_fields_sz_skipn:
+      forall n f,
+        struct_fields_sz (skipn n f) <= struct_fields_sz f.
+    Proof.
+      induction n; simpl; intros; eauto. destr. auto.
+      etransitivity. apply IHn. unfold struct_fields_sz. simpl. lia.
+    Qed.
+    Lemma field_offset_right_le:
+      forall sig s,
+        field_offset_right sig s <= struct_sz sig.
+    Proof.
+      unfold field_offset_right, struct_sz.
+      simpl type_sz.
+      intros; apply struct_fields_sz_skipn.
+    Qed.
+
+    Lemma find_field_offset_right_spec:
+      forall f sig (i: index (List.length (struct_fields sig))),
+        PrimTypeInference.find_field sig f = Success i ->
+        find_field_offset_right (struct_fields sig) f = Some (field_offset_right sig i, field_sz sig i).
+    Proof.
+      intros f sig i FF.
+      unfold PrimTypeInference.find_field in FF. unfold opt_result in FF.
+      destr_in FF; inv FF.
+      revert i Heqo. simpl. destruct sig. simpl. clear.
+      induction struct_fields; intros; eauto. easy.
+      simpl. destruct a. simpl in *.
+      destr_in Heqo.
+      * inv Heqo. f_equal.
+      * destr_in Heqo; inv Heqo.
+        erewrite IHstruct_fields; eauto.
+        f_equal.
+    Qed.
+
+    
+    Lemma usigma1_correct:
       forall ufn fn,
         PrimTypeInference.tc1 ufn (arg1Sig (PrimSignatures.Sigma1 fn)) = Success fn ->
         forall (arg: arg1Sig (PrimSignatures.Sigma1 fn)) ret,
@@ -845,7 +813,7 @@ Lemma usigma1_correct:
     Proof.
       destruct ufn; simpl; intros.
       - destruct fn.
-        + destr_in H; try congruence. inv H. simpl in *. inv Heqr0. subst. reflexivity.
+        + destr_in H; try congruence. inv H. simpl in *. inv Heqr. subst. reflexivity.
         + subst. inv H.
           revert arg. rewrite <- H1. simpl. 
           intro arg. reflexivity.
@@ -859,7 +827,7 @@ Lemma usigma1_correct:
           rewrite uvalue_of_bits_val_of_value. simpl. auto.
         + inv H. revert arg. rewrite <- H2. simpl.
           intros. f_equal.
-      - subst. destr_in H. inv H. simpl in *. inv Heqr0.
+      - subst. destr_in H. inv H. simpl in *. inv Heqr.
         revert arg. rewrite <- H0. simpl. destruct fn; simpl in *; intros.
         + rewrite map_length. rewrite vect_to_list_length. f_equal.
           f_equal. rewrite <- vect_to_list_map. f_equal.
@@ -930,11 +898,11 @@ Lemma usigma1_correct:
         + inv H.
       - destr_in H.
         + repeat destr_in H; inv H.
-          simpl in Heqr0. clear Heqr0. simpl in arg.
+          simpl in Heqr. clear Heqr. simpl in arg.
           simpl PrimSpecs.sigma1.
           simpl.
-          unfold PrimTypeInference.find_field in Heqr1. unfold opt_result in Heqr1.
-          destr_in Heqr1; inv Heqr1.
+          unfold PrimTypeInference.find_field in Heqr0. unfold opt_result in Heqr0.
+          destr_in Heqr0; inv Heqr0.
           revert s0 Heqo arg. destruct s. simpl. clear.
           induction struct_fields; intros; eauto. easy.
           destruct a. destruct arg.
@@ -947,48 +915,12 @@ Lemma usigma1_correct:
         + destr_in H; inv H.
           simpl PrimSpecs.sigma1.
           simpl.
-
-          assert (
-              forall sig (i: index (List.length (struct_fields sig))),
-              PrimTypeInference.find_field sig f = Success i ->
-              find_field_offset_right (struct_fields sig) f = Some (field_offset_right sig i, field_sz sig i)
-            ).
-          {
-            clear. intros sig i FF.
-            unfold PrimTypeInference.find_field in FF. unfold opt_result in FF.
-            destr_in FF; inv FF.
-            revert i Heqo. simpl. destruct sig. simpl. clear.
-            induction struct_fields; intros; eauto. easy.
-            simpl. destruct a. simpl in *.
-            destr_in Heqo.
-            * inv Heqo. f_equal.
-            * destr_in Heqo; inv Heqo.
-              erewrite IHstruct_fields; eauto.
-              f_equal.
-          }
-          erewrite H; eauto. simpl. destr. destr. simpl. f_equal.
+          erewrite find_field_offset_right_spec; eauto. simpl. destr. destr. simpl. f_equal.
           unfold take_drop' in Heqp.
           edestruct (@take_drop_succeeds) as (la & lb & EQ).
           2: rewrite EQ in Heqp.
           rewrite vect_to_list_length.
 
-          Lemma struct_fields_sz_skipn:
-            forall n f,
-              struct_fields_sz (skipn n f) <= struct_fields_sz f.
-          Proof.
-            induction n; simpl; intros; eauto. destr. auto.
-            etransitivity. apply IHn. unfold struct_fields_sz. simpl. lia.
-          Qed.
-          Lemma field_offset_right_le:
-            forall sig s,
-              field_offset_right sig s <= struct_sz sig.
-          Proof.
-            unfold field_offset_right, struct_sz.
-            simpl type_sz.
-
-            intros; apply struct_fields_sz_skipn.
-
-          Qed.
           apply field_offset_right_le.
           f_equal.
           rewrite app_length. rewrite repeat_length.
@@ -1005,20 +937,20 @@ Lemma usigma1_correct:
           unfold take_drop' at 2. rewrite EQ. simpl.
           inv Heqp. rewrite Heqp0. simpl. f_equal. f_equal.
           eapply take_drop'_spec2 in Heqp0. destruct Heqp0.
-          rewrite H1.
-          clear H0 H1.
+          rewrite H0.
+          clear H0.
           eapply take_drop_spec in EQ. intuition.
           rewrite H3. rewrite vect_to_list_length. reflexivity.
       - destr_in H.
         + repeat destr_in H; inv H. simpl in *.
           rewrite <- vect_nth_map. rewrite <- vect_to_list_map.
           rewrite <- vect_to_list_nth. f_equal.
-          unfold PrimTypeInference.check_index in Heqr1.
-          unfold opt_result in Heqr1. destr_in Heqr1; inv Heqr1.
-          symmetry; apply index_to_nat_of_nat. auto.
-        + destr_in H; inv H. simpl in *. destr. destr. simpl.
           unfold PrimTypeInference.check_index in Heqr0.
           unfold opt_result in Heqr0. destr_in Heqr0; inv Heqr0.
+          symmetry; apply index_to_nat_of_nat. auto.
+        + destr_in H; inv H. simpl in *. destr. destr. simpl.
+          unfold PrimTypeInference.check_index in Heqr.
+          unfold opt_result in Heqr. destr_in Heqr; inv Heqr.
           apply index_to_nat_of_nat in Heqo. subst.
           unfold take_drop' in *.
           edestruct @take_drop_succeeds as (la & lb & EQ). 2: rewrite EQ in Heqp.
@@ -1086,36 +1018,35 @@ Lemma usigma1_correct:
       left; subst; reflexivity.
     Defined.
 
+    Lemma strong_ind_type:
+      forall (P: nat -> Type)
+             (IH: forall n, (forall m, m < n -> P m) -> P n),
+      forall n, forall m, m <= n -> P m.
+    Proof.
+      induction n. intros. apply IH. lia.
+      intros.
+      destruct (le_dec m n); eauto.
+      assert (m = S n) by lia. clear H n0. subst.
+      apply IH. intros. apply IHn; auto. lia.
+    Qed.
+
     Lemma val_ind':
       forall (P : val -> Type)
-       (Hbits: forall (n : nat) (bs : list bool), P (Bits n bs))
-       (Henum: forall (sig : enum_sig) (bs : list bool),
-           P (Enum sig bs))
-       (Hstruct: forall (sig : struct_sig) (lv : list val),
-           (forall x, In x lv -> P x) ->
-        P (Struct sig lv))
-       (Harray: forall (sig : array_sig) (lv : list val),
-           (forall x, In x lv -> P x) ->
-        P (Array sig lv)),
+             (Hbits: forall (n : nat) (bs : list bool), P (Bits n bs))
+             (Henum: forall (sig : enum_sig) (bs : list bool),
+                 P (Enum sig bs))
+             (Hstruct: forall (sig : struct_sig) (lv : list val),
+                 (forall x, In x lv -> P x) ->
+                 P (Struct sig lv))
+             (Harray: forall (sig : array_sig) (lv : list val),
+                 (forall x, In x lv -> P x) ->
+                 P (Array sig lv)),
       forall (v : val), P v.
     Proof.
       intros P Hbits Henum Hstruct Harray v.
       remember (size_val v).
       revert v Heqn.
       pattern n.
-
-      Lemma strong_ind_type:
-        forall (P: nat -> Type)
-               (IH: forall n, (forall m, m < n -> P m) -> P n),
-        forall n, forall m, m <= n -> P m.
-      Proof.
-        induction n. intros. apply IH. lia.
-        intros.
-        destruct (le_dec m n); eauto.
-        assert (m = S n) by lia. clear H n0. subst.
-        apply IH. intros. apply IHn; auto. lia.
-      Qed.
-
       eapply strong_ind_type. 2: reflexivity.
       intros n0 Plt v Heqn.
       assert (Plt':
@@ -1179,53 +1110,837 @@ Lemma usigma1_correct:
         left; subst. reflexivity.
     Defined.
 
-    (* Definition ubits2_sigma (ub: ubits2) (v1 v2: list bool) : list bool := *)
-    (*   match ubits2 with *)
-    (*   | UAnd =>  *)
+    Fixpoint bitwise (f: bool -> bool -> bool) (l1 l2: list bool) {struct l1}: list bool :=
+      match l1, l2 with
+      | [], [] => []
+      | [], l2 => map (fun x => f false x) l2
+      | l1, [] => map (fun x => f x false) l1
+      | a1::l1, a2::l2 => f a1 a2 :: bitwise f l1 l2
+      end.
 
-  Definition sigma2 (fn: ufn2) (v1 v2: val) : option val :=
-    match fn with
-    | UEq false  => if val_eq_dec v1 v2 then Bits 1 [true] else Bits 1 [false]
-    | UEq true  => if val_eq_dec v1 v2 then Bits 1 [false] else Bits 1 [true]
-    | UBits2 fn => 
-    | Struct2 SubstField sig idx => fun s v => subst_field sig.(struct_fields) s idx v
-    | Array2 SubstElement sig idx => fun a e => vect_replace a idx e
-    end.
+    Lemma and_correct:
+      forall sz (arg1: arg1Sig (PrimSignatures.Sigma2 (PrimTyped.Bits2 (PrimTyped.And sz))))
+             (arg2: arg2Sig (PrimSignatures.Sigma2 (PrimTyped.Bits2 (PrimTyped.And sz)))) ret,
+        PrimSpecs.sigma2 (PrimTyped.Bits2 (PrimTyped.And sz)) arg1 arg2 = ret ->
+        match val_of_value arg1, val_of_value arg2 with
+        | Bits _ arg1, Bits _ arg2 =>
+          exists sz, Bits sz (bitwise andb arg1 arg2) = (val_of_value ret)
+        | _, _ => False
+        end.
+    Proof.
+      simpl. intros. eexists. f_equal. subst.
+      revert arg1 arg2.
+      induction sz; simpl. reflexivity.
+      destruct arg1, arg2. simpl.
+      unfold Bits.and in *. simpl.
+      rewrite vect_to_list_cons. f_equal. rewrite <- IHsz.
+      reflexivity.
+    Qed.
 
+
+    Lemma len_to_list: forall sz (v: bits sz), sz = Datatypes.length (vect_to_list v).
+    Proof.
+      intros; rewrite vect_to_list_length. reflexivity.
+    Defined.
+
+    Lemma vect_to_list_of_list:
+      forall (v: list bool),
+        vect_to_list (vect_of_list v) = v.
+    Proof.
+      induction v; simpl; intros. reflexivity.
+      rewrite vect_to_list_cons. congruence.
+    Qed.
+
+    Lemma vect_of_list_to_list:
+      forall sz (v: bits sz),
+        vect_of_list (vect_to_list v) = rew [vect bool] (len_to_list sz v) in v.
+    Proof.
+      intros. apply vect_to_list_inj.
+      rewrite vect_to_list_of_list.
+      rewrite vect_to_list_eq_rect. reflexivity.
+    Qed.
+
+
+    Lemma vect_to_list_vect_unsnoc:
+      forall sz (v: bits (S sz)) b v',
+        vect_unsnoc v = (b, v') ->
+        vect_to_list v' = removelast (vect_to_list v).
+    Proof.
+      induction sz; simpl; intros.
+      - inv H. destruct v. simpl. reflexivity.
+      - destr_in H. inv H.
+        rewrite vect_to_list_cons. f_equal.
+        erewrite IHsz. 2: eauto. simpl. reflexivity.
+    Qed.
+
+
+    Lemma lsl1:
+      forall sz (v: bits sz),
+        sz <> 0 ->
+        vect_to_list (Bits.lsl1 v) = false :: removelast (vect_to_list v).
+    Proof.
+      unfold Bits.lsl1. destruct sz. congruence. intros.
+      rewrite vect_to_list_cons. f_equal.
+      erewrite vect_to_list_vect_unsnoc. 2: apply surjective_pairing.
+      reflexivity.
+    Qed.
+
+    Lemma lsl1':
+      forall sz (v: bits sz),
+        vect_to_list (Bits.lsl1 v) = if eq_dec sz O then [] else false :: removelast (vect_to_list v).
+    Proof.
+      intros. destr.
+      subst. destruct v; reflexivity.
+      apply lsl1; auto.
+    Qed.
+
+
+    Definition ubits2_sigma (ub: ubits2) (v1 v2: list bool) : list bool :=
+      match ub with
+      | UAnd => bitwise andb v1 v2
+      | UOr => bitwise orb v1 v2
+      | UXor => bitwise xorb v1 v2
+      | ULsl =>
+        let amount := Bits.to_nat (vect_of_list v2) in
+        Nat.iter amount (fun v =>
+                           if eq_dec (List.length v1) O then [] else false :: removelast v) v1
+      | ULsr =>
+        let amount := Bits.to_nat (vect_of_list v2) in
+        Nat.iter amount (fun v =>
+                           if eq_dec (List.length v1) O then [] else tl v ++ [false]) v1
+      | UAsr =>
+        let amount := Bits.to_nat (vect_of_list v2) in
+        Nat.iter amount (fun v =>
+                           if eq_dec (List.length v1) O then [] else tl v ++ [last v false]) v1
+      | UConcat =>
+        v2 ++ v1
+      | USel =>
+        [List.nth (Bits.to_nat (vect_of_list v2)) v1 false]
+      | USliceSubst ofs w =>
+        let '(h, _) := take_drop' ofs v1 in
+        let '(_, t) := take_drop' (ofs + w) v1 in
+        fst (take_drop' (List.length v1) (h ++ v2 ++ t))
+      | UIndexedSlice w =>
+        let ofs := Bits.to_nat (vect_of_list v2) in
+        let '(_, bs) := take_drop' ofs v1 in
+        let '(bs, _) := take_drop' w bs in
+        (bs ++ List.repeat false (w - Nat.min w (List.length v1 - ofs)))
+      | UPlus =>
+        vect_to_list (Bits.of_N (List.length v1) (Bits.to_N (vect_of_list v1) + Bits.to_N (vect_of_list v2)))
+      | UMinus =>
+        vect_to_list (Bits.of_N (List.length v1)
+                                (Bits.to_N (Bits.of_N (List.length v1) (Bits.to_N (vect_of_list v1) + Bits.to_N (Bits.neg (vect_of_list v2)))) + Bits.to_N (sz:=List.length v1) Bits.one))
+
+      | UMul =>
+        vect_to_list (Bits.of_N (List.length v1 + List.length v2) (Bits.to_N (vect_of_list v1) * Bits.to_N (vect_of_list v2)))
+      | UCompare signed c =>
+        let sz1 := List.length v1 in
+        let sz2 := List.length v2 in
+        match eq_dec sz2 sz1 with
+        | left pf =>
+          let v1 := vect_of_list v1 in
+          let v2 := rew [Bits.bits] pf in vect_of_list v2 in
+              [((if signed
+                 then
+                   match c with
+                   | cLt =>  Bits.signed_lt
+                   | cGt =>  Bits.signed_gt
+                   | cLe =>  Bits.signed_le
+                   | cGe =>  Bits.signed_ge
+                   end
+                 else
+                   match c with
+                   | cLt =>  Bits.unsigned_lt
+                   | cGt =>  Bits.unsigned_gt
+                   | cLe =>  Bits.unsigned_le
+                   | cGe =>  Bits.unsigned_ge
+                   end) v1 v2)]
+        | _ => []
+        end
+
+      end.
+
+    Import PrimTyped.
+
+    Lemma and_correct':
+      forall sz (arg1: bits_t sz)
+             (arg2: bits_t sz),
+        bitwise andb (vect_to_list arg1) (vect_to_list arg2) = vect_to_list (Bits.and arg1 arg2).
+    Proof.
+      induction sz; simpl. reflexivity.
+      destruct arg1, arg2. simpl.
+      unfold Bits.and in *. simpl.
+      rewrite vect_to_list_cons. f_equal. rewrite <- IHsz.
+      reflexivity.
+    Qed.
+
+
+    Lemma or_correct':
+      forall sz (arg1: bits_t sz)
+             (arg2: bits_t sz),
+        bitwise orb (vect_to_list arg1) (vect_to_list arg2) = vect_to_list (Bits.or arg1 arg2).
+    Proof.
+      induction sz; simpl. reflexivity.
+      destruct arg1, arg2. simpl.
+      unfold Bits.or in *. simpl.
+      rewrite vect_to_list_cons. f_equal. rewrite <- IHsz.
+      reflexivity.
+    Qed.
+
+
+    Lemma xor_correct':
+      forall sz (arg1: bits_t sz)
+             (arg2: bits_t sz),
+        bitwise xorb (vect_to_list arg1) (vect_to_list arg2) = vect_to_list (Bits.xor arg1 arg2).
+    Proof.
+      induction sz; simpl. reflexivity.
+      destruct arg1, arg2. simpl.
+      unfold Bits.xor in *. simpl.
+      rewrite vect_to_list_cons. f_equal. rewrite <- IHsz.
+      reflexivity.
+    Qed.
+
+    Lemma iter_assoc_spec:
+      forall {A:Type} (f: A -> A) n x,
+        Nat.iter n f (f x) = f (Nat.iter n f x).
+    Proof.
+      induction n; simpl; intros; eauto.
+      rewrite IHn. auto.
+    Qed.
+    
+    Lemma vect_dotimes_spec:
+      forall {A:Type} (f: A -> A) n x,
+        vect_dotimes f n x = Nat.iter n f x.
+    Proof.
+      induction n; simpl; intros. auto.
+      rewrite IHn, iter_assoc_spec. auto.
+    Qed.
+
+    Lemma vect_to_list_snoc:
+      forall sz (v: bits sz) x,
+        vect_to_list (vect_snoc x v) = vect_to_list v ++ [x].
+    Proof.
+      induction sz; simpl; intros; eauto.
+      rewrite vect_to_list_cons. f_equal.
+      rewrite IHsz. reflexivity.
+    Qed.
+    
+    Lemma lsr1:
+      forall sz (v: bits sz),
+        sz <> 0 ->
+        vect_to_list (Bits.lsr1 v) = tl (vect_to_list v) ++ [false].
+    Proof.
+      unfold Bits.lsr1. intros. destr.
+      rewrite vect_to_list_snoc.
+      rewrite <- (vect_cons_hd_tl v) at 2.
+      rewrite vect_to_list_cons. simpl. reflexivity.
+    Qed.
+
+    Lemma asr1:
+      forall sz (v: bits sz),
+        sz <> 0 ->
+        vect_to_list (Bits.asr1 v) = tl (vect_to_list v) ++ [last (vect_to_list v) false].
+    Proof.
+      unfold Bits.asr1. intros. destr.
+      rewrite vect_to_list_snoc. f_equal.
+      rewrite msb_spec. auto.
+    Qed.
+    
+    Lemma iter_list_vect:
+      forall sz (v: bits sz) (f: list bool -> list bool) (g: bits sz -> bits sz),
+        (forall x, f (vect_to_list x) = vect_to_list (g x)) ->
+        forall n,
+          Nat.iter n f (vect_to_list v) = vect_to_list (vect_dotimes g n v).
+    Proof.
+      intros. rewrite vect_dotimes_spec. induction n; simpl; intros; eauto.
+      rewrite IHn. apply H.
+    Qed.
+
+    Lemma sel:
+      forall sz (bs: bits sz) idx,
+        vect_to_list (BitFuns.sel bs idx) =
+        [List.nth (Bits.to_nat idx) (vect_to_list bs) false].
+    Proof.
+      unfold BitFuns.sel. intros.
+      destr.
+      rewrite bits_nth_list. unfold Bits.to_index in Heqo.
+      erewrite index_to_nat_of_nat. 2: eauto. reflexivity.
+      unfold Bits.to_index in Heqo.
+      rewrite nth_overflow. reflexivity.
+      rewrite vect_to_list_length.
+      apply index_of_nat_none_ge in Heqo. lia.
+    Qed.
+    Lemma slice_subst:
+      forall sz (bs: bits sz) ofs w v,
+        vect_to_list (Bits.slice_subst ofs w bs v) =
+        let '(h, _) := take_drop' ofs (vect_to_list bs) in
+        let '(_, t) := take_drop' (ofs + w) (vect_to_list bs) in
+        fst (take_drop' sz (h ++ (vect_to_list v) ++ t)).
+    Proof.
+      unfold Bits.slice_subst. intros.
+      destr. destr.
+      rewrite vect_to_list_eq_rect.
+      rewrite vect_firstn_to_list. f_equal.
+      rewrite ! vect_to_list_app.
+      rewrite vect_firstn_to_list. f_equal.
+      rewrite Heqp. simpl. f_equal.
+      rewrite vect_skipn_to_list. rewrite Heqp0. reflexivity.
+    Qed.
+
+    Lemma slice:
+      forall sz (bs: bits sz) ofs w,
+        vect_to_list (Bits.slice ofs w bs) =
+        let '(_, bs) := take_drop' ofs (vect_to_list bs) in
+        let '(bs, _) := take_drop' w bs in
+        (bs ++ List.repeat false (w - Nat.min w (sz - ofs))).
+    Proof.
+      intros. unfold Bits.slice. rewrite vect_extend_end_firstn.
+      unfold Bits.extend_end.
+      rewrite vect_to_list_eq_rect.
+      rewrite vect_to_list_app.
+      rewrite vect_firstn_to_list.
+      rewrite vect_skipn_to_list.
+      rewrite <- repeat_bits_const.
+      destr. simpl. destr. simpl.
+      f_equal.
+    Qed.
+    Lemma vect_to_list_eq:
+      forall sz1 sz2 (v1: bits sz1) (v2: bits sz2) (pf: sz1 = sz2),
+        rew [fun x => bits x] pf in v1 = v2 ->
+                                    vect_to_list v1 = vect_to_list v2.
+    Proof.
+      intros. subst. rewrite vect_to_list_eq_rect. auto.
+    Qed.
+
+    Lemma bits_map_rew:
+      forall sz1 sz2 (v: bits sz1) f (pf: sz1 = sz2),
+        Bits.map f (rew [Bits.bits] pf in v) = rew [Bits.bits] pf in (Bits.map f v).
+    Proof.
+      intros. subst. simpl. auto.
+    Qed.
+
+    Lemma cmp:
+      forall sz (v1 v2: bits sz) c,
+        vect_to_list (BitFuns.bitfun_of_predicate c v1 v2) =
+        [c v1 v2].
+    Proof.
+      unfold BitFuns.bitfun_of_predicate. simpl; intros. reflexivity.
+    Qed.
+    Lemma lift_comparison_rew:
+      forall {A} sz1 sz1' (pf: sz1 = sz1') (pf2: sz1 = sz1') (v1: bits sz1) (v2: bits sz1) (cast: forall sz, bits sz -> A) compare cmp,
+        Bits.lift_comparison (cast sz1') compare cmp (rew [Bits.bits] pf in v1) (rew [Bits.bits] pf2 in v2) =
+        Bits.lift_comparison (cast sz1) compare cmp v1 v2.
+    Proof.
+      intros. subst. simpl.
+      rewrite (Eqdep_dec.UIP_refl_nat _ pf2). simpl. reflexivity.
+    Qed.
+
+    Lemma ubits2_correct:
+      forall
+        ub b sz1 sz2
+        (UB:
+           match ub with
+           | USel => Sel sz1
+           | USliceSubst offset width => SliceSubst sz1 offset width
+           | UIndexedSlice width => IndexedSlice sz1 width
+           | UAnd => And sz1
+           | UOr => Or sz1
+           | UXor => Xor sz1
+           | ULsl => Lsl sz1 sz2
+           | ULsr => Lsr sz1 sz2
+           | UAsr => Asr sz1 sz2
+           | UConcat => Concat sz1 sz2
+           | UPlus => Plus sz1
+           | UMinus => Minus sz1
+           | UMul => Mul sz1 sz2
+           | UCompare signed c => Compare signed c sz1
+           end = b)
+        (arg1: arg1Sig (PrimSignatures.Sigma2 (PrimTyped.Bits2 b)))
+        (arg2: arg2Sig (PrimSignatures.Sigma2 (PrimTyped.Bits2 b))) ret,
+        CircuitPrimSpecs.sigma2 b arg1 arg2 = ret ->
+        match val_of_value arg1, val_of_value arg2 with
+        | Bits _ arg1, Bits _ arg2 =>
+          (ubits2_sigma ub arg1 arg2) = (vect_to_list ret)
+        | _, _ => False
+        end.
+    Proof.
+      simpl. intros. subst.
+      destruct ub; simpl in *.
+      apply and_correct'.
+      apply or_correct'.
+      apply xor_correct'.
+      - unfold BitFuns.lsl. unfold Bits.lsl.
+        rewrite vect_of_list_to_list. unfold Bits.to_nat; rewrite Bits.to_N_rew.
+        apply iter_list_vect.
+        intros. rewrite vect_to_list_length. destr. subst. reflexivity.
+        rewrite lsl1; auto.
+      - unfold BitFuns.lsr, Bits.lsr.
+        rewrite vect_of_list_to_list. unfold Bits.to_nat; rewrite Bits.to_N_rew.
+        apply iter_list_vect.
+        intros. rewrite vect_to_list_length. destr. subst. reflexivity.
+        rewrite lsr1; auto.
+      - unfold BitFuns.asr, Bits.asr.
+        rewrite vect_of_list_to_list. unfold Bits.to_nat; rewrite Bits.to_N_rew.
+        apply iter_list_vect.
+        intros. rewrite vect_to_list_length. destr. subst. reflexivity.
+        rewrite asr1; auto.
+      - rewrite vect_to_list_app; auto.
+      - rewrite sel.
+        rewrite vect_of_list_to_list. unfold Bits.to_nat; rewrite Bits.to_N_rew. auto.
+      - rewrite vect_to_list_length.
+        rewrite slice_subst. reflexivity.
+      - rewrite slice.
+        rewrite vect_of_list_to_list. unfold Bits.to_nat; rewrite Bits.to_N_rew.
+        destr. destr. f_equal. f_equal. rewrite vect_to_list_length. reflexivity.
+      - unfold Bits.plus.
+        rewrite ! vect_of_list_to_list.
+        rewrite ! Bits.to_N_rew.
+        eapply vect_to_list_eq.
+        erewrite (f_equal_dep _ (fun x => Bits.of_N x (Bits.to_N arg1 + Bits.to_N arg2))).
+        Unshelve. 2: apply vect_to_list_length.
+        auto.
+      - unfold Bits.minus.
+        rewrite ! vect_of_list_to_list.
+        rewrite ! Bits.to_N_rew.
+        eapply vect_to_list_eq.
+        erewrite (f_equal_dep _ (fun x => Bits.of_N x _)).
+        Unshelve. 2: apply vect_to_list_length.
+        unfold Bits.plus. f_equal.
+        f_equal.
+        replace (Bits.neg (rew [Bits.bits] len_to_list sz1 arg2 in arg2))
+          with (rew [Bits.bits] len_to_list sz1 arg2 in (Bits.neg arg2)).
+        rewrite Bits.to_N_rew.
+        erewrite <- (f_equal_dep _ (fun x => (Bits.of_N x _))).
+        Unshelve. 5: apply len_to_list.
+        rewrite Bits.to_N_rew. auto.
+        unfold Bits.neg.
+        rewrite bits_map_rew. reflexivity.
+        erewrite <- Bits.to_N_rew.
+        Unshelve. 3: apply vect_to_list_length.
+        f_equal.
+        apply f_equal_dep.
+      - unfold Bits.mul.
+        rewrite ! vect_of_list_to_list.
+        rewrite ! Bits.to_N_rew.
+        eapply vect_to_list_eq.
+        erewrite (f_equal_dep _ (fun x => Bits.of_N x (Bits.to_N arg1 * Bits.to_N arg2))).
+        Unshelve. 2: rewrite ! vect_to_list_length; auto.
+        auto.
+      - destr.
+        + rewrite ! vect_of_list_to_list.
+          rewrite rew_compose.
+          transitivity ( vect_to_list
+                           (BitFuns.bitfun_of_predicate (if signed
+                                                         then
+                                                           match c with
+                                                           | cLt =>  Bits.signed_lt
+                                                           | cGt =>  Bits.signed_gt
+                                                           | cLe =>  Bits.signed_le
+                                                           | cGe =>  Bits.signed_ge
+                                                           end
+                                                         else
+                                                           match c with
+                                                           | cLt =>  Bits.unsigned_lt
+                                                           | cGt =>  Bits.unsigned_gt
+                                                           | cLe =>  Bits.unsigned_le
+                                                           | cGe =>  Bits.unsigned_ge
+                                                           end) arg1 arg2)
+                       ). 2: repeat destr; reflexivity.
+          rewrite cmp. f_equal.
+          repeat destr; apply lift_comparison_rew.
+        + clear -n. exfalso.
+          rewrite ! vect_to_list_length in n. congruence.
+    Qed.
+
+
+    (*   Definition sigma2 (fn: PrimTyped.fbits2) : CSig_denote (CircuitSignatures.CSigma2 fn) := *)
+    (*     match fn with *)
+    (*     | Sel _ => sel *)
+    (*     | SliceSubst _ offset width => Bits.slice_subst offset width *)
+    (*     | IndexedSlice _ width => fun bs offset => Bits.slice (Bits.to_nat offset) width bs *)
+    (*     | And _ => Bits.and *)
+    (*     | Or _ => Bits.or *)
+    (*     | Xor _ => Bits.xor *)
+    (*     | Lsl _ _ => lsl *)
+    (*     | Lsr _ _ => lsr *)
+    (*     | Asr _ _ => asr *)
+    (*     | Concat _ _ => Bits.app *)
+    (*     | Plus _ => Bits.plus *)
+    (*     | Minus _ => Bits.minus *)
+    (*     | Mul _ _ => Bits.mul *)
+    (*     | EqBits _ false => _eq *)
+    (*     | EqBits _ true => _neq *)
+    (*     | Compare true cLt _ => bitfun_of_predicate Bits.signed_lt *)
+    (*     | Compare true cGt _ => bitfun_of_predicate Bits.signed_gt *)
+    (*     | Compare true cLe _ => bitfun_of_predicate Bits.signed_le *)
+    (*     | Compare true cGe _ => bitfun_of_predicate Bits.signed_ge *)
+    (*     | Compare false cLt _ => bitfun_of_predicate Bits.unsigned_lt *)
+    (*     | Compare false cGt _ => bitfun_of_predicate Bits.unsigned_gt *)
+    (*     | Compare false cLe _ => bitfun_of_predicate Bits.unsigned_le *)
+    (*     | Compare false cGe _ => bitfun_of_predicate Bits.unsigned_ge *)
+    (*     end. *)
+
+    Fixpoint subst_field (n: nat) (v: val) (s: list val) : option (list val) :=
+      match n, s with
+      | _, [] => None
+      | O, a::r => Some (v::r)
+      | S n, a::r => let/opt s := subst_field n v r in Some (a::s)
+      end.
+
+    Fixpoint val_of_struct_value'
+             (fields : list (string * type))
+             (x : struct_denote fields)
+             {struct fields} : list val :=
+      match fields as fields0 return (struct_denote fields0 -> list val) with
+      | [] => fun _ : unit => []
+      | p :: fields0 =>
+        let (_, tau) as p0 return (snd p0 * struct_denote fields0 -> list val) := p in
+        fun '(x0, xs) => val_of_value x0 :: val_of_struct_value' fields0 xs
+      end x.
+
+    Lemma val_of_struct_value_rew:
+      forall fields x,
+        (fix
+           val_of_struct_value (fields : list (string * type)) (x : struct_denote fields) {struct
+                                                                                             fields} : list val :=
+           match fields as fields0 return (struct_denote fields0 -> list val) with
+           | [] => fun _ : unit => []
+           | p :: fields0 =>
+             let (_, tau) as p0 return (snd p0 * struct_denote fields0 -> list val) := p in
+             fun '(x0, xs) => val_of_value x0 :: val_of_struct_value fields0 xs
+           end x) fields x =
+        val_of_struct_value' fields x.
+    Proof.
+      induction fields; simpl; intros; eauto.
+    Qed.
+
+    Lemma subst_field_ok':
+      forall flds idx v s,
+        subst_field (index_to_nat idx) (val_of_value v)
+                    (val_of_struct_value' flds s) =
+        Some (val_of_struct_value' flds
+                                   (BitFuns.subst_field flds s idx v)).
+    Proof.
+      induction flds; simpl; intros; eauto. easy.
+      repeat destr. simpl in *. auto.
+      simpl in *. rewrite IHflds. simpl. auto.
+    Qed.
+
+    Lemma subst_field_ok:
+      forall sig idx (s: struct_t sig) v,
+        exists s',
+          val_of_value s = Struct sig s' /\
+          exists s'',
+          subst_field (index_to_nat idx) (val_of_value v) s' = Some s'' /\
+          Struct sig s'' =
+          val_of_value (tau:=struct_t sig) (BitFuns.subst_field (struct_fields sig) s idx v)
+    .
+    Proof.
+      intros.
+      simpl in s.
+      revert s idx v. simpl. intros.
+      rewrite ! val_of_struct_value_rew.
+      eexists; split; eauto.
+      rewrite subst_field_ok'.
+      eexists; split; eauto.
+    Qed.
+
+    Fixpoint subst_field_name (flds: list (string * type)) (n: string)
+             (v: val) (s: list val) : option (list val) :=
+      match flds, s with
+      | _, [] => None
+      | [], _ => None
+      | (name, _)::flds, a::r =>
+        if eq_dec n name then Some (v::r)
+        else let/opt s := subst_field_name flds n v r in Some (a::s)
+      end.
+
+
+    Lemma subst_field_name_ok':
+      forall flds x idx fname v s,
+            PrimTypeInference.find_field {| struct_name := x; struct_fields := flds|} fname = Success idx ->
+        subst_field_name flds fname (val_of_value v)
+                    (val_of_struct_value' flds s) =
+        Some (val_of_struct_value' flds
+                                   (BitFuns.subst_field flds s idx v)).
+    Proof.
+      induction flds; simpl; intros; eauto. easy.
+      destr_in v.
+      - destruct a. destruct s. simpl in *.
+        unfold PrimTypeInference.find_field in H. simpl in H.
+        destr_in H.
+        + subst. simpl in H. inv H. auto.
+        + destr_in H; inv H.
+      - destruct a, s.
+        unfold PrimTypeInference.find_field in H. simpl in H.
+        destr_in H.
+        + subst. simpl in H. inv H.
+        + destr_in H; inv H. simpl in *. erewrite IHflds with (x:=x). simpl. auto.
+          unfold PrimTypeInference.find_field. simpl. rewrite Heqo. simpl. auto.
+    Qed.
+
+    Lemma subst_field_name_ok:
+      forall sig fname idx (s: struct_t sig) v,
+        PrimTypeInference.find_field sig fname = Success idx ->
+        exists s',
+          val_of_value s = Struct sig s' /\
+          exists s'',
+          subst_field_name (struct_fields sig) fname (val_of_value v) s' = Some s'' /\
+          Struct sig s'' =
+          val_of_value (tau:=struct_t sig) (BitFuns.subst_field (struct_fields sig) s idx v)
+    .
+    Proof.
+      intros.
+      simpl in s.
+      revert s idx v H. simpl. intros.
+      rewrite ! val_of_struct_value_rew.
+      eexists; split; eauto.
+      erewrite subst_field_name_ok'.
+      eexists; split; eauto.
+      instantiate(1:= struct_name sig).
+      destruct sig. eauto.
+    Qed.
+
+    Lemma vect_replace_to_list:
+      forall {A: Type} sz (v: vect A sz) l1 (a: A) l2 x idx,
+        vect_to_list v = l1 ++ a :: l2 ->
+        List.length l1 = index_to_nat idx ->
+        vect_to_list (vect_replace v idx x) = l1 ++ x :: l2.
+    Proof.
+      induction sz; simpl; intros; eauto. easy.
+      destr.
+      - destruct l1; simpl in *; try lia. subst.
+        rewrite vect_to_list_cons. f_equal.
+        destruct v; simpl in *.
+        unfold vect_to_list in H. simpl in H. inv H. reflexivity.
+      - rewrite vect_to_list_cons. subst. simpl.
+        destruct v; simpl in *.
+        unfold vect_to_list in H. simpl in H. fold (@vect_to_list A) in H.
+        destruct l1. simpl in *. lia. simpl in H. inv H.
+        simpl. f_equal. simpl in H0. inv H0.
+        eapply IHsz; eauto.
+    Qed.
+
+    Lemma take_drop_map:
+      forall {A B: Type} (f: A -> B) n l l1 l2,
+        take_drop n (map f l) = Some (l1, l2) ->
+        exists l1' l2',
+          take_drop n l = Some (l1', l2') /\
+          l1 = List.map f l1' /\
+          l2 = List.map f l2'.
+    Proof.
+      induction n; simpl; intros; eauto.
+      - inv H. exists [], l; repeat split; eauto.
+      - destr_in H. inv H.
+        destruct (take_drop n l0) eqn:?; try congruence. 2: inv H.
+        destruct p; simpl in *. inv H.
+        destr. simpl in *. congruence. simpl in *. inv Heql0.
+        edestruct IHn as (l1' & l2' & EQ1 & EQ2 & EQ3). eauto.
+        rewrite EQ1. simpl. (do 2 eexists); repeat split; eauto.
+        subst; reflexivity.
+    Qed.
+
+    Definition sigma2 (fn: ufn2) (v1 v2: val) : option val :=
+      match fn with
+      | UEq false  => Some (Bits 1 [if val_eq_dec v1 v2 then true else false])
+      | UEq true  =>  Some (Bits 1 [if val_eq_dec v1 v2 then false else true])
+      | UBits2 fn =>
+        match v1, v2 with
+          Bits _ v1, Bits _ v2 => let res := ubits2_sigma fn v1 v2 in
+                                  Some (Bits (List.length res) res)
+        | _, _ => None
+        end
+      | UStruct2 (USubstField fname) =>
+        match v1 with
+          Struct sig v1 =>
+          let/opt res := subst_field_name (struct_fields sig) fname v2 v1 in
+          Some (Struct sig res)
+        | _ => None
+        end
+      | UStruct2 (USubstFieldBits sig fname) =>
+        match v1, v2 with
+          Bits sz v1, Bits _ v2 =>
+          let/opt2 ofs, w := find_field_offset_right (struct_fields sig) fname in
+          let res := ubits2_sigma (USliceSubst ofs w) v1 v2 in
+          Some (Bits sz res)
+        | _, _ => None
+        end
+      | UArray2 (USubstElement n) =>
+        match v1 with
+          | Array s v1 =>
+            let/opt2 l1, l2 := take_drop n v1 in
+            match l2 with
+              [] => None
+            | a::l2 => Some (Array s (l1 ++ v2 :: l2))
+            end
+          | _ => None
+        end
+      | UArray2 (USubstElementBits sig n) =>
+        match v1, v2 with
+          Bits sz v1, Bits _ v2 =>
+          let res := ubits2_sigma (USliceSubst ((array_len sig - S n) * element_sz sig) (element_sz sig)) v1 v2 in
+          Some (Bits sz res)
+        | _, _ => None
+        end
+      end.
+
+
+    Lemma sigma2_correct:
+          forall ufn fn ty1 ty2,
+            PrimTypeInference.tc2
+              ufn
+              ty1 ty2 = Success fn ->
+            forall (arg1: arg1Sig (PrimSignatures.Sigma2 fn))
+                   (arg2: arg2Sig (PrimSignatures.Sigma2 fn)),
+              sigma2 ufn (val_of_value arg1) (val_of_value arg2) = Some (val_of_value (PrimSpecs.sigma2 fn arg1 arg2)).
+    Proof.
+      destruct ufn; simpl; intros.
+      - inv H. simpl in *. destr; f_equal; f_equal.
+        unfold BitFuns._neq. unfold beq_dec. destruct (eq_dec).
+        subst. destr. reflexivity.
+        destr. 2: reflexivity.
+        exfalso. apply n. apply bits_of_value_inj. apply vect_to_list_inj.
+        erewrite ! (ubits_of_value_ok _ _ eq_refl). rewrite e. reflexivity.
+        unfold BitFuns._eq. unfold beq_dec. destruct (eq_dec).
+        subst. destr. reflexivity.
+        destr. 2: reflexivity.
+        exfalso. apply n. apply bits_of_value_inj. apply vect_to_list_inj.
+        erewrite ! (ubits_of_value_ok _ _ eq_refl). rewrite e. reflexivity.
+      - destr_in H. 2: congruence.
+        destr_in Heqr; try congruence.
+        destr_in H; try congruence.
+        destr_in Heqr0; try congruence.
+        inv Heqr0. inv Heqr. inv H.
+        generalize (ubits2_correct fn _ s s0 eq_refl arg1 arg2 _ eq_refl).
+        destr; try easy.
+        destr; try easy. intro A; rewrite A. simpl.
+        rewrite vect_to_list_length. simpl. auto.
+      - destr_in H.
+        + destr_in H; try congruence.
+          destr_in Heqr; try congruence.
+          destr_in H; try congruence.
+          inv Heqr. inv H. simpl in arg1, arg2.
+          edestruct subst_field_name_ok as (s' & VOV & s'' & SFN & EQ). eauto.
+          rewrite VOV. rewrite SFN. simpl.
+          rewrite ! val_of_struct_value_rew.
+          f_equal. rewrite EQ. simpl.
+          rewrite val_of_struct_value_rew.
+          reflexivity.
+        + subst. destr_in H; try congruence. inv H. simpl in *.
+          rewrite slice_subst.
+          erewrite find_field_offset_right_spec; eauto. simpl.
+          rewrite vect_to_list_length. reflexivity.
+      - destr.
+        + destr_in H; try congruence.
+          destr_in H; inv H. destr_in Heqr; inv Heqr. simpl in *.
+          assert (pos < array_len s).
+          {
+            destruct (lt_dec pos (array_len s)). auto.
+            unfold PrimTypeInference.check_index in Heqr0. unfold opt_result in Heqr0.
+            destr_in Heqr0; inv Heqr0.
+            rewrite index_of_nat_ge_none in Heqo. congruence. lia.
+          }
+          edestruct @take_drop_succeeds as (l1 & l2 & EQ).
+          2: rewrite EQ.
+          rewrite map_length. rewrite vect_to_list_length. lia. simpl.
+
+          edestruct (@take_drop_map) as (l1' & l2' & EQ4 & EQ5 & EQ6). eauto.
+
+          edestruct (@take_drop_spec) as (EQ1 & EQ2 & EQ3). apply EQ4.
+          rewrite vect_to_list_length in EQ3.
+          destr. erewrite <- map_length in EQ3. rewrite <- EQ6 in EQ3. simpl in EQ3. lia.
+
+          destruct l2'; simpl in *; try congruence. inv EQ6.
+          erewrite vect_replace_to_list; eauto.
+          rewrite map_app. reflexivity.
+          unfold PrimTypeInference.check_index in Heqr0. unfold opt_result in Heqr0.
+          destr_in Heqr0; inv Heqr0.
+          symmetry; eapply index_to_nat_of_nat; eauto.
+
+        + destr_in H; try congruence. inv H. simpl in *.
+          rewrite slice_subst.
+          unfold PrimTypeInference.check_index in Heqr. unfold opt_result in Heqr.
+          destr_in Heqr; inv Heqr.
+          unfold element_offset_right.
+          erewrite index_to_nat_of_nat; eauto.
+          rewrite Bits.rmul_correct.
+          rewrite vect_to_list_length. reflexivity.
+    Qed.
+
+    Context (r: REnv.(env_t) (fun _ => val)).
+    Context (sigma: forall f: ext_fn_t, val -> val).
+
+    Section Args.
+      Context (interp_action:
+                 forall (Gamma: list (var_t * val))
+                        (sched_log: Log) (action_log: Log)
+                        (a: uaction),
+                   option (Log * val * (list (var_t * val)))).
+
+      Fixpoint interp_args'
+               (Gamma: list (var_t * val))
+               (sched_log: Log)
+               (action_log: Log)
+               (argspec: tsig var_t)
+               (args: list uaction)
+        : option (Log * list (var_t * val) * list (var_t * val)) :=
+        match argspec, args with
+        | [], [] => Some (action_log, [], Gamma)
+        | argspec:: argspecs, arg :: args =>
+          let/opt3 action_log, ctx, Gamma := interp_args' Gamma sched_log action_log argspecs args in
+          let/opt3 action_log, v, Gamma := interp_action Gamma sched_log action_log arg in
+          Some (action_log, (fst argspec,v)::ctx, Gamma)
+        | _, _ => None
+        end.
+    End Args.
+
+    Fixpoint list_assoc {K V: Type} {eq: EqDec K} (l: list (K * V)) (k: K): option V :=
+      match l with
+        [] => None
+      | (k1,v1)::l =>
+        if eq_dec k k1 then Some v1 else list_assoc  l k
+      end.
+
+    Fixpoint list_assoc_set {K V: Type} {eq: EqDec K} (l: list (K * V)) (k: K) (v: V): list (K * V) :=
+      match l with
+        [] => [(k,v)]
+      | (k1,v1)::l =>
+        if eq_dec k k1 then (k1,v)::l else (k1,v1) :: list_assoc_set l k v
+      end.
 
     Fixpoint interp_action
-             {sig: tsig var_t}
-             (Gamma: tcontext sig)
+             (Gamma: list (var_t * val))
              (sched_log: Log)
              (action_log: Log)
              (a: uaction)
              {struct a}
-      : option (Log * val * (tcontext sig)) :=
+      : option (Log * val * list (var_t * val)) :=
       match a with
       | UError e => None
+      | UFail _ => None
       | USugar _ => None
       | UVar var =>
-        let/opt v := ucassoc Gamma var in
+        let/opt v := list_assoc Gamma var in
         Some (action_log, v, Gamma)
       | @UConst _ _ _ _ _ tau cst =>
-        Some (action_log, val_of_type_cst _ cst, Gamma)
+        Some (action_log, val_of_value cst, Gamma)
       | UAssign k a =>
         let/opt3 action_log, v, Gamma := interp_action Gamma sched_log action_log a in
-        Some (action_log, Bits _ Ob, replace k v Gamma)
+        Some (action_log, Bits 0 [], list_assoc_set Gamma k v)
       | USeq a1 a2 =>
         let/opt3 action_log, v, Gamma := interp_action Gamma sched_log action_log a1 in
         interp_action Gamma sched_log action_log a2
       | UBind k a1 a2 =>
-        let/opt3 action_log, v, Gamma
-          := interp_action Gamma sched_log action_log a1 in
-        let/opt3 action_log, v, Gamma := interp_action
-          (CtxCons (k, bits_t 0) v Gamma) sched_log action_log a2
-        in Some (action_log, v, ctl Gamma)
+        let/opt3 action_log, v, Gamma :=
+           interp_action Gamma sched_log action_log a1 in
+        let/opt3 action_log, v, Gamma :=
+           interp_action ((k, v):: Gamma) sched_log action_log a2
+        in Some (action_log, v, tl Gamma)
       | UIf cond athen aelse =>
         let/opt3 action_log, v, Gamma := interp_action Gamma sched_log action_log cond in
         match v with
-        | Bits 1 b =>
-          if Bits.single b then
+        | Bits 1 [b] =>
+          if b then
             interp_action Gamma sched_log action_log athen
           else
             interp_action Gamma sched_log action_log aelse
@@ -1233,45 +1948,874 @@ Lemma usigma1_correct:
         end
       | URead prt idx =>
         if may_read sched_log prt idx then
-          Some (log_cons idx (LE LogRead prt (Bits 0 (vect_nil))) action_log,
+          Some (log_cons idx (LE LogRead prt (Bits 0 [])) action_log,
                 match prt with
                 | P0 => REnv.(getenv) r idx
                 | P1 => match latest_write0 (V:=val) (log_app action_log sched_log) idx with
-                       | Some v => v
-                       | None => REnv.(getenv) r idx
-                       end
+                        | Some v => v
+                        | None => REnv.(getenv) r idx
+                        end
                 end,
                 Gamma)
         else None
       | UWrite prt idx v =>
         let/opt3 action_log, val, Gamma := interp_action Gamma sched_log action_log v in
         if may_write sched_log action_log prt idx then
-          Some (log_cons idx (LE LogWrite prt val) action_log, Bits _ Bits.nil, Gamma)
+          Some (log_cons idx (LE LogWrite prt val) action_log, Bits 0 [], Gamma)
         else None
       | UUnop fn arg =>
         let/opt3 action_log, arg1, Gamma := interp_action Gamma sched_log action_log arg in
-        Some (action_log, (PrimSpecs.sigma1 fn) arg1, Gamma)
-      | _ => None
-      end.
-
-      | Unop fn arg1 => fun Gamma =>
-        let/opt3 action_log, arg1, Gamma := interp_action Gamma sched_log action_log arg1 in
-        Some (action_log, (PrimSpecs.sigma1 fn) arg1, Gamma)
-      | Binop fn arg1 arg2 => fun Gamma =>
+        let/opt v := sigma1 fn arg1 in
+        Some (action_log, v, Gamma)
+      | UBinop fn arg1 arg2 =>
         let/opt3 action_log, arg1, Gamma := interp_action Gamma sched_log action_log arg1 in
         let/opt3 action_log, arg2, Gamma := interp_action Gamma sched_log action_log arg2 in
-        Some (action_log, (PrimSpecs.sigma2 fn) arg1 arg2, Gamma)
-      | ExternalCall fn arg1 => fun Gamma =>
+        let/opt v := sigma2 fn arg1 arg2 in
+        Some (action_log, v, Gamma)
+      | UExternalCall fn arg1 =>
         let/opt3 action_log, arg1, Gamma := interp_action Gamma sched_log action_log arg1 in
         Some (action_log, sigma fn arg1, Gamma)
-      | InternalCall name args body => fun Gamma =>
-        let/opt3 action_log, results, Gamma := interp_args' (@interp_action) Gamma sched_log action_log args in
-        let/opt3 action_log, v, _ := interp_action results sched_log action_log body in
+      | UInternalCall f args =>
+        let body := int_body f in
+        let/opt3 action_log, results, Gamma :=
+           fold_right (fun a acc =>
+                        let/opt3 action_log, l, Gamma := acc in
+                        let/opt3 action_log, v, Gamma :=
+                           interp_action Gamma sched_log action_log a in
+                        Some (action_log, v::l, Gamma))
+                     (Some (action_log, [], Gamma)) args in
+        let/opt3 action_log, v, _ :=
+           interp_action
+             (map (fun '(name, _, v) => (name, v))
+                  (combine (int_argspec f) results)) sched_log action_log body in
         Some (action_log, v, Gamma)
-      | APos _ a => fun Gamma =>
+      | UAPos p a =>
         interp_action Gamma sched_log action_log a
-      end Gamma.
+      end.
+    End Action.
+End Interp.
 
+Section Eq.
+      Require TypedSemantics.
+
+      Require TypeInference.
+
+  Context {pos_t var_t fn_name_t reg_t ext_fn_t: Type}.
+  Context {reg_t_eq_dec: EqDec reg_t}.
+  Context {var_t_eq_dec: EqDec var_t}.
+
+      
+      Context {TR: reg_t -> type}.
+  Context {Sigma: ext_fn_t -> ExternalSignature}.
+  Context {REnv: Env reg_t}.
+      Context (r: env_t REnv (fun x : reg_t => val)).
+      Context (sigma: forall f: ext_fn_t, val -> val).
+      Context (tr: env_t REnv (fun x : reg_t => TR x)).
+      Context (tsigma: forall f, Sig_denote (Sigma f)).
+
+      Hypothesis tsigma_correct:
+        forall f v,
+          sigma f (val_of_value v) = val_of_value (tsigma f v).
+
+      Definition env_t_R
+                 {K: Type}
+                 {V1 V2: K -> Type}
+                 (R: forall k, V1 k -> V2 k -> Prop)
+                 (e: Env K)
+                 (e1: env_t e (fun x => V1 x))
+                 (e2: env_t e (fun x => V2 x)) : Prop :=
+        forall k,
+          R k (getenv e e1 k) (getenv e e2 k).
+
+      Definition logentrykind_eq (uk: LogEntryKind) (k: Logs.LogEntryKind) :=
+        match uk, k with
+        | LogRead, Logs.LogRead => True
+        | LogWrite, Logs.LogWrite => True
+        | _, _ => False
+        end.
+      
+      (* Definition logentry_eq {V:type} (url: LogEntry val) (rl: Logs.LogEntry V) : Prop. *)
+      (*   destruct url, rl. *)
+      (*   destruct kind0. exact True. *)
+      (*   exact (val0 = val_of_value val1). *)
+      (*   Set Printing All. *)
+      (*   Show Proof. *)
+
+      Definition logentry_eq {V:type} (ule: LogEntry val) (le: Logs.LogEntry V) : Prop :=
+        logentrykind_eq (kind ule) (Logs.kind le) /\
+        port ule = Logs.port le /\
+        match Logs.kind le as l return
+              (match l return Type with
+               | Logs.LogRead => unit
+               | Logs.LogWrite => type_denote V
+               end -> Prop) with
+          | Logs.LogRead => fun _ => ULogs.val ule = Bits 0 []
+          | Logs.LogWrite => fun v => ULogs.val ule = val_of_value v
+        end (Logs.val le).
+
+      Definition rlog_eq {V:type} (url: RLog val) (rl: Logs.RLog V) :=
+        Forall2 (fun ule le => logentry_eq ule le) url rl.
+
+      Notation Log := (@_ULog val reg_t REnv).
+
+      (* Notation rule := (rule pos_t var_t fn_name_t R Sigma). *)
+      Notation uaction := (uaction pos_t var_t fn_name_t reg_t ext_fn_t).
+      (* Notation scheduler := (scheduler pos_t rule_name_t). *)
+
+
+      Definition log_eq REnv (ul: env_t REnv (fun _ => RLog val)) (l: Logs.Log TR REnv) : Prop :=
+        env_t_R (V1:= fun k => Logs.RLog (TR k))
+                        (V2:= fun k => RLog val)
+                        (fun k v1 v2 => rlog_eq v2 v1) REnv l ul.
+
+      Inductive gamma_eq :
+        forall (sig: tsig var_t), list (var_t * val) -> TypedSemantics.tcontext sig -> Prop :=
+      | gamma_eq_nil:
+          gamma_eq [] [] (CtxEmpty)
+      | gamma_eq_cons:
+          forall sig k t v ug g,
+            gamma_eq sig ug g ->
+            gamma_eq ((k,t)::sig) ((k,val_of_value v)::ug) (@CtxCons _ _ _ (k,t) v g)
+      .
+
+
+      (* Definition gamma_eq {sig} (UGamma: list (var_t * val)) *)
+      (*            (Gamma: TypedSemantics.tcontext sig) : Prop := *)
+      (*   forall k t (m: member _ sig), *)
+      (*     assoc k sig = Some (existT _ t m) -> *)
+      (*     Some (val_of_value (cassoc m Gamma)) =  (list_assoc UGamma k). *)
+
+
+      Lemma gamma_eq' {sig} (UGamma: list (var_t * val))
+                 (Gamma: TypedSemantics.tcontext sig) :
+        gamma_eq sig UGamma Gamma ->
+        forall k t (m: member _ sig),
+          assoc k sig = Some (existT _ t m) ->
+          Some (val_of_value (cassoc m Gamma)) =  (list_assoc UGamma k).
+      Proof.
+        induction 1; simpl; intros; eauto. congruence. simpl in *.
+        repeat destr_in H0; simpl in *; subst.
+        unfold eq_rect_r in H0; simpl in H0.
+        inv H0.
+        apply Eqdep_dec.inj_pair2_eq_dec in H3. subst. 2: apply eq_dec.
+        simpl. auto.
+        inv H0.
+        apply Eqdep_dec.inj_pair2_eq_dec in H3. subst. 2: apply eq_dec.
+        simpl. eauto.
+        inv H0.
+      Qed.
+
+      
+      Lemma cast_action'_eq:
+        forall (p: pos_t) (sig: tsig var_t) (tau1 tau2: type)
+               (a: TypedSyntax.action pos_t var_t fn_name_t TR Sigma sig tau1)
+               (e: error_message var_t fn_name_t) a',
+          TypeInference.cast_action' TR Sigma p tau2 a e = Success a' ->
+          exists p : tau1 = tau2,
+            a' = eq_rect _ _ a _ p.
+      Proof.
+        unfold TypeInference.cast_action'. intros.
+        destr_in H. subst.
+        unfold eq_rect_r in H. simpl in H. inv H.
+        exists eq_refl; reflexivity. inv H.
+      Qed.
+
+      Lemma cast_action_eq:
+        forall (p: pos_t) (sig: tsig var_t) (tau1 tau2: type)
+               (a: TypedSyntax.action pos_t var_t fn_name_t TR Sigma sig tau1)
+               a',
+          TypeInference.cast_action TR Sigma p tau2 a = Success a' ->
+          exists p : tau1 = tau2,
+            a' = eq_rect _ _ a _ p.
+      Proof.
+        intros. unfold TypeInference.cast_action in H.
+        eapply cast_action'_eq; eauto.
+      Qed.
+
+
+
+      Lemma list_assoc_gss:
+        forall {K V: Type} (eq: EqDec K) (l: list (K * V)) k v,
+          list_assoc (list_assoc_set l k v) k = Some v.
+      Proof.
+        induction l; simpl; intros; eauto.
+        destr.
+        repeat destr; eauto.
+        simpl. rewrite Heqs. auto.
+        simpl. rewrite Heqs. eauto.
+      Qed.
+
+      Lemma list_assoc_gso:
+        forall {K V: Type} (eq: EqDec K) (l: list (K * V)) k k' v (d: k <> k'),
+          list_assoc (list_assoc_set l k v) k' = list_assoc l k'.
+      Proof.
+        induction l; simpl; intros; eauto.
+        destr.
+        repeat destr; simpl; eauto.
+        - rewrite Heqs0. auto.
+        - rewrite Heqs0. auto.
+        - rewrite Heqs0. eauto.
+      Qed.
+
+      Lemma gamma_eq_replace:
+        forall sig g1 g2
+               (Geq: gamma_eq sig g1 g2)
+               k t v
+               (m: member (k, t) sig)
+               (ASSOC: assoc k sig = Some (existT (fun k2 : type => member (k, k2) sig) t m)),
+
+          gamma_eq sig (list_assoc_set g1 k (val_of_value v))
+                   (creplace m v g2).
+      Proof.
+        induction 1; simpl; intros; eauto. congruence.
+        repeat destr_in ASSOC; simpl in *; try congruence.
+        - subst. unfold eq_rect_r in ASSOC; simpl in ASSOC.
+          inv ASSOC.
+          apply Eqdep_dec.inj_pair2_eq_dec in H1. subst. 2: apply eq_dec.
+          simpl.
+          constructor. auto.
+        - inv ASSOC.
+          apply Eqdep_dec.inj_pair2_eq_dec in H1. subst. 2: apply eq_dec.
+          simpl.
+          constructor. eauto.
+      Qed.
+
+      (*       Lemma gamma_eq_replace: *)
+      (*   forall sig (* (ND: NoDup (map fst sig)) *) g1 g2 k t v *)
+      (*          (m: member (k, t) sig) *)
+      (*          (ASSOC: assoc k sig = Some (existT (fun k2 : type => member (k, k2) sig) t m)), *)
+      (*     gamma_eq g1 g2 -> *)
+      (*     gamma_eq (list_assoc_set g1 k (val_of_value v)) *)
+      (*              (creplace m v g2). *)
+      (* Proof. *)
+      (*   unfold gamma_eq. simpl. intros. *)
+      (*   destruct (eq_dec k k0). *)
+      (*   - subst. *)
+      (*     rewrite H0 in ASSOC; inv ASSOC. *)
+      (*     apply Eqdep_dec.inj_pair2_eq_dec in H3. subst. 2: apply eq_dec. *)
+      (*     rewrite cassoc_creplace_eq. *)
+      (*     rewrite list_assoc_gss. auto. *)
+      (*   - rewrite cassoc_creplace_neq_k; auto. *)
+      (*     rewrite list_assoc_gso. eauto. auto. intro A; inv A. congruence. *)
+      (* Qed. *)
+
+
+
+      Lemma log_eq_existsb:
+        forall usched_log sched_log,
+          log_eq REnv usched_log sched_log ->
+          forall idx f uf,
+            (forall ule idx le,
+                logentrykind_eq ule le ->
+                uf ule idx = f le idx
+            ) ->
+            Logs.log_existsb sched_log idx f =
+            log_existsb usched_log idx uf.
+      Proof.
+        unfold Logs.log_existsb, log_existsb. intros.
+        unfold log_eq in H. red in H.
+        red in H.
+        generalize (H idx).
+        generalize (@getenv _ REnv (fun x => Logs.RLog (TR x)) sched_log idx).
+        generalize (getenv REnv usched_log idx).
+        clear - H0.
+        induction 1; simpl; intros. auto.
+        red in H. intuition.
+        destruct x, y; simpl in *. subst.
+        erewrite H0; eauto. f_equal. eauto.
+      Qed.
+
+      Lemma may_read_eq:
+        forall usched_log sched_log,
+          log_eq REnv usched_log sched_log ->
+          forall port idx,
+            Logs.may_read sched_log port idx =
+            may_read usched_log port idx.
+      Proof.
+        unfold Logs.may_read, may_read.
+        intros.
+        rewrite ! log_eq_existsb with (f:=Logs.is_write0) (uf:=is_write0) (usched_log:=usched_log); auto.
+        rewrite ! log_eq_existsb with (f:=Logs.is_write1) (uf:=is_write1) (usched_log:=usched_log); auto.
+        destruct ule, le; simpl; auto; try easy.
+        destruct ule, le; simpl; auto; try easy.
+      Qed.
+
+
+      Lemma log_eq_app:
+        forall ul1 ul2 l1 l2,
+          log_eq REnv ul1 l1 ->
+          log_eq REnv ul2 l2 ->
+          log_eq REnv (log_app ul1 ul2) (Logs.log_app l1 l2).
+      Proof.
+        unfold log_app, Logs.log_app.
+        unfold log_eq. unfold env_t_R.
+        simpl. intros.
+        rewrite ! getenv_map2.
+        apply Forall2_app; eauto.
+        apply H. apply H0.
+      Qed.
+
+      Lemma may_write_eq:
+        forall usched_log sched_log,
+          log_eq REnv usched_log sched_log ->
+          forall urule_log rule_log,
+            log_eq REnv urule_log rule_log ->
+            forall port idx,
+              Logs.may_write sched_log rule_log port idx =
+              may_write usched_log urule_log port idx.
+      Proof.
+        unfold Logs.may_write, may_write.
+        intros.
+        generalize (log_eq_app _ _ _ _ H0 H).
+        intros.
+        rewrite ! log_eq_existsb with (f:=Logs.is_write0) (uf:=is_write0) (usched_log:=log_app urule_log usched_log); auto.
+        rewrite ! log_eq_existsb with (f:=Logs.is_write1) (uf:=is_write1) (usched_log:=log_app urule_log usched_log); auto.
+        rewrite ! log_eq_existsb with (f:=Logs.is_read1) (uf:=is_read1) (usched_log:=log_app urule_log usched_log); auto.
+        destruct ule, le; simpl; auto; try easy.
+        destruct ule, le; simpl; auto; try easy.
+        destruct ule, le; simpl; auto; try easy.
+      Qed.
+
+
+
+      Lemma log_find_eq:
+        forall ulog log,
+          log_eq REnv ulog log ->
+          forall idx,
+          forall f uf,
+            (forall ule (le: Logs.LogEntry (TR idx)),
+                logentry_eq ule le ->
+                uf ule = option_map (val_of_value) (f le)
+            ) ->
+
+            option_map (val_of_value (tau:=TR idx)) (Logs.log_find log idx f) =
+            (log_find ulog idx uf).
+      Proof.
+        unfold Logs.log_find, log_find.
+        intros.
+        red in H. red in H. red in H.
+        generalize (H idx).
+        generalize (@getenv _ REnv (fun x => Logs.RLog (TR x)) log idx).
+        generalize (getenv REnv ulog idx).
+        clear - H0.
+        induction 1; simpl; intros. auto.
+        erewrite H0; eauto. destr; simpl; eauto.
+      Qed.
+
+      Lemma latest_write0_eq:
+        forall ulog log,
+          log_eq REnv ulog log ->
+          forall idx,
+            option_map (val_of_value (tau:=TR idx)) (Logs.latest_write0 log idx) =
+            (latest_write0 ulog idx).
+      Proof.
+        unfold Logs.latest_write0, latest_write0.
+        intros.
+        eapply log_find_eq. auto.
+        intros. red in H0. intuition.
+        destruct ule, le; simpl in *. subst.
+        destr_in val1.
+        - subst. red in H1. destr; try easy.
+        - subst. red in H1. destr; try easy.
+          destr; auto.
+      Qed.
+
+      Lemma log_eq_cons:
+        forall idx ulog (log: Logs._Log) ule le,
+          log_eq REnv ulog log ->
+          logentry_eq ule le ->
+          log_eq REnv (log_cons idx ule ulog) (Logs.log_cons idx le log).
+      Proof.
+        unfold log_eq. unfold env_t_R.
+        unfold rlog_eq.
+        intros. unfold log_cons, Logs.log_cons.
+        destruct (eq_dec idx k).
+        - subst.
+          rewrite ! get_put_eq.
+          constructor; eauto.
+        - rewrite ! get_put_neq; eauto.
+      Qed.
+
+      
+
+      Hypothesis r_eq:
+        forall i,
+          getenv REnv r i = val_of_value (getenv REnv tr i).
+
+      Lemma interp_action_correct:
+        forall ua p sig tau a
+               (TA: TypeInference.type_action TR Sigma p sig ua = Success (existT _ tau a))
+               (Gamma: TypedSemantics.tcontext sig)
+               (UGamma: list (var_t * val))
+               (GammaEq: gamma_eq sig UGamma Gamma)
+               sched_log action_log action_log'
+               usched_log uaction_log
+               (SL: log_eq REnv usched_log sched_log)
+               (AL: log_eq REnv uaction_log action_log)
+               v Gamma'
+        ,
+          TypedSemantics.interp_action
+            tr tsigma
+            Gamma sched_log action_log a = Some (action_log', v, Gamma') ->
+          exists uaction_log' UGamma',
+            interp_action
+              (pos_t:=pos_t)
+              (fn_name_t := fn_name_t)
+              r sigma UGamma usched_log uaction_log ua = Some (uaction_log', val_of_value v, UGamma')
+            /\ log_eq REnv uaction_log' action_log'
+            /\ gamma_eq sig UGamma' Gamma'
+      .
+      Proof.
+        fix IHua 1.
+        destruct ua; simpl; intros.
+        - inv TA.
+        - inv TA.
+          apply Eqdep_dec.inj_pair2_eq_dec in H2. subst.
+          simpl in H. inv H.
+          apply eq_dec.
+        - destr_in TA; inv TA.
+          apply Eqdep_dec.inj_pair2_eq_dec in H2. 2: apply eq_dec. subst.
+          simpl in H. inv H.
+          unfold opt_result in Heqr0; destr_in Heqr0; inv Heqr0. destruct s.
+          simpl.
+          setoid_rewrite <- gamma_eq'. simpl.
+          exists uaction_log, UGamma; split; eauto. eauto. eauto.
+        - inv TA.
+          apply Eqdep_dec.inj_pair2_eq_dec in H2. 2: apply eq_dec. subst.
+          simpl in H. inv H.
+          exists uaction_log, UGamma; split; eauto.
+        - destr_in TA; [|inv TA].
+          destr_in TA; [|inv TA].
+          destr_in TA; [|inv TA]. inv TA.
+          apply Eqdep_dec.inj_pair2_eq_dec in H2. 2: apply eq_dec. subst. simpl in H.
+          unfold opt_bind in H.
+          destr_in H; [|inv H].
+          destr_in H. destr_in H. inv H.
+          unfold opt_result in Heqr0; destr_in Heqr0; inv Heqr0. destruct s. simpl in *.
+          destruct s0. simpl in *.
+          apply cast_action_eq in Heqr2.
+          destruct Heqr2 as (pf & EQ). subst.
+          simpl in Heqo.
+          edestruct (IHua ua _ _ _ _ Heqr1) as (ual' & g' & IA' & ALeq & Geq). auto.
+          4: apply Heqo. eauto. eauto. eauto.
+          rewrite IA'. simpl.
+          eexists; eexists; repeat split; eauto.
+          apply gamma_eq_replace; eauto.
+        - destr_in TA; [|inv TA].
+          destr_in TA; [|inv TA].
+          destr_in TA; [|inv TA]. inv TA.
+          apply Eqdep_dec.inj_pair2_eq_dec in H2. 2: apply eq_dec. subst. simpl in H.
+          unfold opt_bind in H.
+          destr_in H; [|inv H].
+          destr_in H. destr_in H.
+          destruct s. simpl in *.
+          apply cast_action_eq in Heqr1.
+          destruct Heqr1 as (pf & EQ). subst.
+          simpl in Heqo.
+          edestruct (IHua ua1 _ _ _ _ Heqr0) as (ual' & g' & IA' & ALeq & Geq). auto.
+          4: apply Heqo. eauto. eauto. eauto.
+          rewrite IA'. simpl.
+          destruct s1. simpl in *.
+          edestruct (IHua ua2 _ _ _ _ Heqr2) as (ual2' & g2' & IA2' & ALeq2 & Geq2). auto.
+          4: apply H. eauto. eauto. eauto.
+          rewrite IA2'.
+          eexists; eexists; repeat split; eauto.
+        - destr_in TA; [|inv TA].
+          destr_in TA; [|inv TA].
+          inv TA.
+          apply Eqdep_dec.inj_pair2_eq_dec in H2. 2: apply eq_dec. subst. simpl in H.
+          unfold opt_bind in H.
+          destr_in H; [|inv H].
+          destr_in H. destr_in H. destr_in H; [|inv H].
+          destruct p2. destruct p2. inv H.
+          destruct s, s0. simpl in *.
+          edestruct (IHua ua1 _ _ _ _ Heqr0) as (ual' & g' & IA' & ALeq & Geq). auto.
+          4: apply Heqo. eauto. eauto. eauto.
+          rewrite IA'. simpl.
+          edestruct (IHua ua2 _ _ _ _ Heqr1 (CtxCons (v,x) t0 t) ((v,val_of_value t0)::g')) as (ual2' & g2' & IA2' & ALeq2 & Geq2).
+          4: apply Heqo0. 2-3: eauto.
+          constructor; auto.
+          rewrite IA2'. simpl.
+          eexists; eexists; repeat split; eauto. inv Geq2.
+          apply Eqdep_dec.inj_pair2_eq_dec in H4. 2: apply eq_dec. subst. simpl. auto.
+        - destr_in TA; [|inv TA].
+          destr_in TA; [|inv TA].
+          destr_in TA; [|inv TA].
+          destr_in TA; [|inv TA].
+          destr_in TA; [|inv TA].
+          inv TA.
+          apply Eqdep_dec.inj_pair2_eq_dec in H2. 2: apply eq_dec. subst. simpl in H.
+          unfold opt_bind in H.
+          destr_in H; [|inv H].
+          destruct p0. destruct p0.
+          destruct s. simpl in *.
+          apply cast_action_eq in Heqr1.
+          destruct Heqr1 as (pf & EQ). subst.
+          simpl in Heqo.
+          edestruct (IHua ua1 _ _ _ _ Heqr0) as (ual' & g' & IA' & ALeq & Geq).
+          4: apply Heqo. eauto. eauto. eauto.
+          rewrite IA'. simpl.
+          destruct s1, s2. simpl in *.
+          apply cast_action_eq in Heqr4.
+          destruct Heqr4 as (pf & EQ). subst.
+          simpl in H.
+          destr.
+          + edestruct (IHua ua2 _ _ _ _ Heqr2) as (ual2' & g2' & IA2' & ALeq2 & Geq2).
+            4: apply H. eauto. eauto. eauto.
+            rewrite IA2'. simpl.
+            eexists; eexists; repeat split; eauto.
+          + edestruct (IHua ua3 _ _ _ _ Heqr3) as (ual2' & g2' & IA2' & ALeq2 & Geq2).
+            4: apply H. eauto. eauto. eauto.
+            rewrite IA2'. simpl.
+            eexists; eexists; repeat split; eauto.
+        - inv TA.
+          apply Eqdep_dec.inj_pair2_eq_dec in H2. 2: apply eq_dec. subst. simpl in H.
+          erewrite may_read_eq in H; eauto.
+          destr_in H; [|inv H]. inv H.
+          eexists; eexists; repeat split; eauto.
+          f_equal. f_equal. f_equal.
+          rewrite ! r_eq.
+          destr.
+
+          erewrite <- latest_write0_eq; eauto.
+          2: apply log_eq_app; eauto.
+          destruct (Logs.latest_write0) eqn:?; simpl; auto.
+
+          apply log_eq_cons; auto.
+          red. simpl. auto.
+        - destr_in TA; [|inv TA].
+          destr_in TA; [|inv TA].
+          inv TA.
+          apply Eqdep_dec.inj_pair2_eq_dec in H2. 2: apply eq_dec. subst. simpl in H.
+          unfold opt_bind in H.
+          destr_in H; [|inv H].
+          destruct p0. destruct p0.
+
+          destruct s. simpl in *.
+          apply cast_action_eq in Heqr1.
+          destruct Heqr1 as (pf & EQ). subst.
+          simpl in Heqo.
+          edestruct (IHua ua _ _ _ _ Heqr0) as (ual' & g' & IA' & ALeq & Geq).
+          4: apply Heqo. eauto. eauto. eauto.
+          rewrite IA'. simpl.
+          erewrite may_write_eq in H; eauto.
+          destr_in H; [|inv H]. inv H.
+          eexists; eexists; repeat split; eauto.
+          apply log_eq_cons; auto.
+          red. simpl. auto.
+        - destr_in TA; [|inv TA].
+          destr_in TA; [|inv TA].
+          destr_in TA; [|inv TA].
+          inv TA.
+          apply Eqdep_dec.inj_pair2_eq_dec in H2. 2: apply eq_dec. subst. simpl in H.
+          unfold opt_bind in H.
+          destr_in H; [|inv H].
+          destruct p0. destruct p0. inv H.
+          destruct s. simpl in *.
+          apply cast_action_eq in Heqr2.
+          destruct Heqr2 as (pf & EQ). subst.
+          simpl in Heqo.
+          edestruct (IHua ua _ _ _ _ Heqr0) as (ual' & g' & IA' & ALeq & Geq).
+          4: apply Heqo. eauto. eauto. eauto.
+          rewrite IA'. simpl.
+          unfold TypeInference.lift_fn1_tc_result in Heqr1.
+          unfold result_map_failure in Heqr1. destr_in Heqr1; inv Heqr1.
+          erewrite usigma1_correct; eauto. simpl.
+          eexists; eexists; repeat split; eauto.
+        - destr_in TA; [|inv TA].
+          destr_in TA; [|inv TA].
+          destr_in TA; [|inv TA].
+          destr_in TA; [|inv TA].
+          destr_in TA; [|inv TA].
+          inv TA.
+          apply Eqdep_dec.inj_pair2_eq_dec in H2. 2: apply eq_dec. subst. simpl in H.
+          unfold opt_bind in H.
+          destr_in H; [|inv H].
+          destruct p0. destruct p0.
+          destr_in H; [|inv H].
+          destruct p0. destruct p0.
+          inv H.
+          destruct s, s0. simpl in *.
+          apply cast_action_eq in Heqr3.
+          destruct Heqr3 as (pf & EQ). subst.
+          simpl in Heqo.
+          apply cast_action_eq in Heqr4.
+          destruct Heqr4 as (pf & EQ). subst.
+          simpl in Heqo0.
+          edestruct (IHua ua1 _ _ _ _ Heqr0) as (ual' & g' & IA' & ALeq & Geq).
+          4: apply Heqo. eauto. eauto. eauto.
+          rewrite IA'. simpl.
+          edestruct (IHua ua2 _ _ _ _ Heqr1) as (ual2' & g2' & IA2' & ALeq2 & Geq2).
+          4: apply Heqo0. eauto. eauto. eauto.
+          rewrite IA2'. simpl.
+          unfold TypeInference.lift_fn2_tc_result in Heqr2.
+          unfold result_map_failure in Heqr2. destr_in Heqr2; inv Heqr2.
+          erewrite sigma2_correct; eauto. simpl.
+          eexists; eexists; repeat split; eauto.
+        - destr_in TA; [|inv TA].
+          destr_in TA; [|inv TA].
+          inv TA.
+          apply Eqdep_dec.inj_pair2_eq_dec in H2. 2: apply eq_dec. subst. simpl in H.
+          unfold opt_bind in H.
+          destr_in H; [|inv H].
+          destruct p0. destruct p0. inv H.
+          destruct s. simpl in *.
+          apply cast_action_eq in Heqr1.
+          destruct Heqr1 as (pf & EQ). subst.
+          simpl in Heqo.
+          edestruct (IHua ua _ _ _ _ Heqr0) as (ual' & g' & IA' & ALeq & Geq).
+          4: apply Heqo. eauto. eauto. eauto.
+          rewrite IA'. simpl.
+          eexists; eexists; repeat split; eauto.
+          rewrite tsigma_correct. eauto.
+        - destr_in TA; [|inv TA].
+          destr_in TA; [|inv TA].
+          destr_in TA; [|inv TA].
+          destr_in TA; [|inv TA].
+          inv TA.
+          apply Eqdep_dec.inj_pair2_eq_dec in H2. 2: apply eq_dec. subst. simpl in H.
+          unfold opt_bind in H.
+          destr_in H; [|inv H].
+          destruct p0. destruct p0. 
+          destr_in H; [|inv H].
+          destruct p0. destruct p0.
+          inv H.
+          destruct s1. simpl in *.
+          apply cast_action_eq in Heqr3.
+          destruct Heqr3 as (pf & EQ). subst.
+          simpl in Heqo0.
+
+          unfold TypeInference.assert_argtypes in Heqr1.
+
+
+    Fixpoint assert_argtypes' {sig}
+             (args_desc: tsig var_t)
+             (args: list (pos_t * {tau : type & TypedSyntax.action pos_t var_t fn_name_t TR Sigma sig tau}))
+      : result (context (K := (var_t * type)) (fun k_tau => TypedSyntax.action pos_t var_t fn_name_t TR Sigma sig (snd k_tau)) args_desc) unit :=
+      match args_desc, args with
+      | [], [] => Success CtxEmpty
+      | [], _ => Failure tt
+      | _, [] => Failure tt
+      | (name1, tau1) :: fn_sig, (pos1, arg1) :: args =>
+        match TypeInference.cast_action TR Sigma pos1 tau1 (projT2 arg1) with
+          Success arg1 =>
+          let/res ctx := assert_argtypes' fn_sig args in
+          Success (CtxCons (name1, tau1) arg1 ctx)
+        | _ => Failure tt
+        end
+      end.
+    Lemma assert_argtypes'_eq : forall {T:Type} (sig: tsig var_t) args_desc args s ufn fname n p,
+      TypeInference.assert_argtypes' (T:=T) TR Sigma ufn n fname p args_desc args = Success s <->
+      assert_argtypes' (sig:=sig) args_desc args = Success s.
+    Proof.
+      induction args_desc; simpl; intros; eauto.
+      - destr; split; intuition congruence.
+      - destruct a. split. intros.
+        + destr_in H; [inv H|]. destr_in H.
+          destr_in H; [|inv H].
+          destr_in H; [|inv H]. inv H.
+          erewrite (proj1 (IHargs_desc _ _ _ _ _ _)). eauto. eauto.
+        + intros. destr_in H; [inv H|]. destr_in H.
+          destr_in H; [|inv H].
+          destr_in H; [|inv H]. inv H.
+          erewrite (proj2 (IHargs_desc _ _ _ _ _ _)). eauto. eauto.
+    Qed.
+
+    rewrite assert_argtypes'_eq in Heqr1.
+
+    Lemma result_list_map_length {A B F: Type} (f: A -> result B F):
+      forall la lb,
+        result_list_map f la = Success lb ->
+        List.length lb = List.length la.
+    Proof.
+      induction la; simpl; intros; eauto. inv H; reflexivity.
+      destr_in H; [|inv H].
+      destr_in H; [|inv H]. inv H.
+      simpl.
+      erewrite IHla; eauto.
+    Qed.
+
+    Lemma result_list_map_app1 {A B F: Type} (f: A -> result B F):
+      forall la1 la2 lb1 lb2,
+        result_list_map f la1 = Success lb1 ->
+        result_list_map f la2 = Success lb2 ->
+        result_list_map f (la1 ++ la2) = Success (lb1 ++ lb2).
+    Proof.
+      induction la1; simpl; intros; eauto. inv H. simpl; auto.
+      destr_in H; [|inv H].
+      destr_in H; [|inv H]. inv H.
+      erewrite IHla1; eauto. simpl; auto.
+    Qed.
+
+    Lemma result_list_map_app2 {A B F: Type} (f: A -> result B F):
+      forall la1 la2 lb,
+        result_list_map f (la1 ++ la2) = Success lb ->
+        exists lb1 lb2,
+          result_list_map f la1 = Success lb1 /\
+          result_list_map f la2 = Success lb2 /\
+          lb = lb1 ++ lb2.
+    Proof.
+      induction la1; simpl; intros; eauto.
+      destr_in H; [|inv H].
+      destr_in H; [|inv H]. inv H.
+      edestruct IHla1 as (lb1 & lb2 & EQ1 & EQ2 & EQl). eauto. subst.
+      rewrite EQ1, EQ2.
+      eexists; eexists; repeat split; eauto.
+    Qed.
+
+    Lemma result_list_map_rev {A B F: Type} (f: A -> result B F):
+      forall la lb,
+        result_list_map f la = Success lb ->
+        result_list_map f (rev la) = Success (rev lb).
+    Proof.
+      induction la; simpl; intros; eauto. inv H; reflexivity.
+      destr_in H; [|inv H].
+      destr_in H; [|inv H]. inv H.
+      simpl.
+      erewrite result_list_map_app1; eauto. simpl. rewrite Heqr0. auto.
+    Qed.
+    
+    assert (List.length args = List.length (rev s)).
+    {
+      apply result_list_map_length in Heqr0. rewrite <- Heqr0.
+      rewrite rev_length; auto.
+    }
+
+    Lemma combine_nil_inv:
+      forall {A B: Type} (la: list A) (lb: list B),
+        List.length la = List.length lb ->
+        combine la lb = [] ->
+        la = [] /\ lb = [].
+    Proof.
+      induction la; simpl; intros.
+      - destruct lb; simpl in *; auto. lia.
+      - destruct lb. simpl in H. lia. inv H0.
+    Qed.
+
+    Lemma rev_nil_inv:
+      forall {A:Type} (l: list A),
+        rev l = [] -> l = [].
+    Proof.
+      destruct l; simpl in *. auto.
+      intros.
+      apply (f_equal (@List.length _)) in H.
+      rewrite app_length in H; simpl in H; lia.
+    Qed.
+
+    Lemma combine_app:
+      forall {A B : Type} (la1 la2 : list A) (lb1 lb2: list B),
+        List.length la1 = List.length lb1 ->
+        List.length la2 = List.length lb2 ->
+        combine (la1 ++ la2) (lb1 ++ lb2) = combine la1 lb1 ++ combine la2 lb2.
+    Proof.
+      induction la1; simpl; intros; eauto.
+      - destruct lb1; simpl in *; try lia. auto.
+      - destruct lb1; simpl in *; try lia.
+        rewrite IHla1 by lia. auto.
+    Qed.
+
+    
+    Lemma combine_rev:
+      forall {A B : Type} (la : list A) (lb: list B),
+        List.length la = List.length lb ->
+        rev (combine la lb) = combine (rev la) (rev lb).
+    Proof.
+      induction la; simpl; intros; eauto.
+      destr. simpl in *; lia. simpl in *.
+      rewrite IHla by lia.
+      rewrite combine_app. simpl. auto.
+      rewrite ! rev_length; lia.
+      simpl; lia.
+    Qed.
+    
+          assert (
+              forall (p : pos_t) (sig : tsig var_t) s,
+                result_list_map (TypeInference.type_action TR Sigma p sig) args = Success s ->
+                forall (Gamma : TypedSemantics.tcontext sig) (UGamma : list (var_t * val)),
+                  gamma_eq sig UGamma Gamma ->
+         forall (sched_log action_log action_log' : Logs.Log TR REnv)
+           (usched_log uaction_log : env_t REnv (fun _ : reg_t => RLog val)),
+         log_eq REnv usched_log sched_log ->
+         log_eq REnv uaction_log action_log ->
+         forall (s0 : context
+         (fun k_tau : var_t * type =>
+          TypedSyntax.action pos_t var_t fn_name_t TR Sigma sig (snd k_tau)) 
+         (rev (int_argspec ufn))),
+           assert_argtypes' (rev (int_argspec ufn))
+                            (rev (combine (map (TypeInference.actpos p) args) s)) = Success s0 ->
+           List.length args = List.length (rev s) ->
+         forall v (Gamma' : TypedSemantics.tcontext sig),
+           TypedSemantics.interp_args'
+             (@TypedSemantics.interp_action pos_t var_t fn_name_t reg_t ext_fn_t TR Sigma REnv tr tsigma)
+             Gamma sched_log action_log s0 = 
+         Some (action_log', v, Gamma') ->
+         exists (uaction_log' : Log) res (UGamma' : list (var_t * val)),
+           fold_right
+          (fun a0 (acc : option (Log * list val * list (var_t * val))) =>
+           let/opt3 action_log0, l0, Gamma0 := acc
+           in (let/opt3 action_log1, v0, Gamma1
+               := interp_action r sigma Gamma0 usched_log action_log0 a0
+               in Some (action_log1, v0 :: l0, Gamma1))) (Some (uaction_log, [], UGamma)) args =
+           Some (uaction_log', res, UGamma') /\
+           gamma_eq _ (combine (map fst (rev (int_argspec ufn))) (rev res)) v /\
+           log_eq REnv uaction_log' action_log' /\ gamma_eq sig UGamma' Gamma').
+          {
+            clear - IHua.
+            rewrite <- (rev_involutive args).
+            generalize (rev args) as args'.
+            intros args' p sig s RLM.
+            apply result_list_map_rev in RLM.
+            rewrite combine_rev.
+            rewrite map_rev. rewrite rev_involutive.
+            revert RLM. rewrite rev_involutive.
+            generalize (rev s) as s'. clear s.
+            revert args' p sig.
+            generalize (rev (int_argspec ufn)). clear args.
+            induction l; simpl; intros.
+            admit. admit. admit.
+            (* - destr_in H3; [|now inv H3]. inv H3. *)
+            (*   apply rev_nil_inv in Heql. *)
+            (*   apply combine_nil_inv in Heql; eauto. destruct Heql. subst. *)
+            (*   rewrite map_rev in H3. *)
+            (*   apply rev_nil_inv in H3. *)
+            (*   destruct args'; simpl in *; try congruence. inv H5. *)
+            (*   eexists; eexists; eexists; repeat split; eauto. *)
+            (*   constructor. *)
+            (*   rewrite <- H4. rewrite map_length. auto. *)
+            (* - destr_in H3. *)
+            (*   destr_in H3; [inv H3|]. *)
+            (*   destr_in H3. *)
+            (*   destr_in H3; [|inv H3]. *)
+            (*   destr_in H3; [|inv H3]. inv H3. *)
+            (*   destruct args'. *)
+            (*   + simpl in H. inv H. simpl in Heql0. congruence. *)
+            (*   + simpl in H. *)
+            (*     destr_in H; [|inv H]. *)
+            (*   destr_in H; [|inv H]. inv H. simpl in *. *)
+            (*   unfold opt_bind in H4. *)
+            (*   destr_in H4; [|inv H4]. destruct p0. destruct p0. *)
+            (*   destr_in H4; [|inv H4]. destruct p0. destruct p0. *)
+            (*   inv H4. simpl in *. *)
+            (*   rewrite fold_left_app. *)
+            (*   edestruct IHl as (ual' & res & ug' & EQ & Geq' & ALeq & Geq2'). *)
+            (*   apply Heqr3. 4: eauto. *)
+          }
+          admit.
+        - destr_in TA; [|inv TA].
+          inv TA.
+          apply Eqdep_dec.inj_pair2_eq_dec in H2. 2: apply eq_dec. subst. simpl in H.
+          destruct s. simpl in *.
+          edestruct (IHua ua _ _ _ _ Heqr0) as (ual' & g' & IA' & ALeq & Geq).
+          4: apply H. eauto. eauto. eauto.
+          rewrite IA'.
+          eexists; eexists; repeat split; eauto.
+        - inv TA.
+      Qed.
+
+      
+
+    End Eq.
+    
     Definition interp_rule (sched_log: Log) (rl: rule) : option Log :=
       match interp_action CtxEmpty sched_log log_empty rl with
       | Some (l, _, _) => Some l
